SystemFD/Metatheory/Classification.lean
@@ -4,7 +4,7 @@ import SystemFD.Judgment
 import SystemFD.Ctx
 import SystemFD.Metatheory.Weaken
 import SystemFD.Metatheory.Substitution
-import SystemFD.Metatheory.Uniqueness
+import SystemFD.Metatheory.FrameWf
 
 @[simp]
 abbrev class_idx (t A : Term) : JudgmentArgs v :=
@@ -13,11 +13,11 @@ abbrev class_idx (t A : Term) : JudgmentArgs v :=
   | .wf => ()
 
 @[simp]
-abbrev ClassType (Γ : Ctx Term) : (v : JudgmentVariant) -> JudgmentArgs v -> Prop
+abbrev ClassificationLemmaType (Γ : Ctx Term) : (v : JudgmentVariant) -> JudgmentArgs v -> Prop
 | .prf => λ (_, A) => A = .kind ∨ (Γ ⊢ A : .kind) ∨ (∃ K, Γ ⊢ K : .kind ∧ Γ ⊢ A : K)
 | .wf => λ () => ∀ x T, Frame.get_type (Γ d@ x) = .some T -> Γ ⊢ T : .kind ∨ (Γ ⊢ T : ★)
 
-theorem classification_lemma : Judgment v Γ ix -> ClassType Γ v ix := by
+theorem classification_lemma : Judgment v Γ ix -> ClassificationLemmaType Γ v ix := by
 intro j; induction j <;> simp at *
 all_goals (try simp [*])
 case wfnil =>
@@ -271,13 +271,13 @@ case _ j1 j2 ih1 ih2 =>
     apply Or.inr; apply Or.inr
     apply Exists.intro ★; apply And.intro
     apply ih2; apply beta_kind q2 j1
-case _ ih =>
+case cast ih =>
   cases ih
   case _ ih => cases ih
   case _ ih =>
   cases ih; case _ K ih =>
   cases ih; case _ ih1 ih2 =>
-  cases ih2; case _ K ih2' _ ih2 =>
+  cases ih2; case _ K _ _ _ _ ih2' _ ih2 =>
     apply Or.inr; apply Or.inr
     apply Exists.intro K; apply And.intro
     apply ih2'; apply ih2
@@ -312,76 +312,108 @@ case _ j1 _ ih1 ih2 =>
     cases ih2; case _ K ih2 =>
     cases ih2; case _ ih2 ih2' =>
     cases ih2'; case _ K2 w1 w2 w3 =>
-      have lem := uniqueness_of_types q3 w2; subst lem
       apply Or.inr; apply Exists.intro ★
       apply And.intro; constructor
       apply judgment_ctx_wf j1
       constructor; apply q1
       apply q2; apply w3
-case _ j1 j2 j3 j4 j5 j6 _ _ ih _ _ _ =>
-  cases ih
-  case _ ih =>
-    cases ih
-    case _ ih1 ih2 =>
-      apply Or.inr; apply Exists.intro ★
-      apply And.intro; constructor
-      apply judgment_ctx_wf j1
-      constructor; apply ih2
-      constructor; apply j1; apply j4
-      constructor; apply j2; apply j5
-  case _ ih =>
-  cases ih; case _ K ih =>
-  cases ih; case _ ih1 ih2 =>
-    cases ih2; cases ih1
-case _ j1 j2 j3 j4 j5 j6 _ _ _ _ _ _ =>
-  apply Or.inr; apply Exists.intro ★
-  apply And.intro; constructor
-  apply judgment_ctx_wf j1
-  apply Judgment.eq _; constructor
-  apply j1; apply j4; constructor
-  apply j2; apply j5; constructor
-  apply judgment_ctx_wf j1
-case _ j1 j2 _ ih _ _ =>
-  cases ih
-  case _ ih =>
-    cases ih; case _ ih1 ih2 =>
-      apply Or.inr; apply Exists.intro ★
-      apply And.intro; constructor
-      apply judgment_ctx_wf j1
-      apply Judgment.eq _; apply j1; apply j2
-      constructor; apply ih1; apply ih2
-  case _ ih =>
-  cases ih; case _ K ih =>
-  cases ih; case _ ih1 ih2 =>
-    cases ih2; cases ih1
-case _ j1 j2 j3 j4 _ _ _ ih =>
-  apply Or.inr; apply Exists.intro ★
-  apply And.intro; constructor
-  apply judgment_ctx_wf j1
-  constructor; apply j1; apply j2
-  apply j3
-case _ j1 j2 _ _ _ _ =>
-  apply Or.inr; apply Exists.intro ★
-  apply And.intro; constructor
-  apply judgment_ctx_wf j1
-  apply Judgment.eq _; apply j1; apply j2
-  constructor; apply judgment_ctx_wf j1
-case _ j1 j2 _ _ _ _ _ ih1 ih2 =>
+case _ Γ t1 K1 K2 A B t2 C D j1 j2 ih1 ih2 =>
+  apply Or.inr
   cases ih1
   case _ ih1 => cases ih1
   case _ ih1 =>
   cases ih1; case _ K ih1 =>
-  cases ih1; case _ ih1 ih3 =>
-  cases ih3; case _ q1 q2 q3 =>
-  cases q2; case _ w1 w2 =>
-  cases q3; case _ r1 r2 =>
-    have lem1 := beta_kind w2 j1; simp at lem1
-    have lem2 := beta_kind r2 j2; simp at lem2
-    apply Or.inr; apply Exists.intro ★
-    apply And.intro; constructor
-    apply judgment_ctx_wf j1
-    apply Judgment.eq _; apply lem1; apply lem2
-    constructor; apply judgment_ctx_wf j1
+  cases ih1; case _ lem1 lem2 =>
+  cases lem2; case _ q1 q2 q3 =>
+  cases ih2
+  case _ ih2 => cases ih2
+  case _ ih2 =>
+  cases ih2; case _ K' ih2 =>
+  cases ih2; case _ lem3 lem4 =>
+  cases lem4; case _ w1 w2 w3 =>
+  cases q1; case _ q1 q4 =>
+    apply Exists.intro ★; apply And.intro lem1
+    apply Judgment.eq q4
+    constructor; apply q2; assumption
+    constructor; apply q3; assumption
+case _ Γ t1 A B t2 C D j1 j2 ih1 ih2 =>
+  apply Or.inr; apply Exists.intro ★
+  cases ih1; case _ ih1 => cases ih1
+  case _ ih1 =>
+  cases ih2; case _ ih2 => cases ih2
+  case _ ih2 =>
+  cases ih1; case _ K1 ih1 =>
+  cases ih1; case _ lem1 lem2 =>
+  cases ih2; case _ K2 ih2 =>
+  cases ih2; case _ lem3 lem4 =>
+  cases lem2; case _ q1 q2 q3 =>
+  cases lem4; case _ w1 w2 w3 =>
+    apply And.intro lem1
+    apply Judgment.eq q1
+    constructor; assumption; assumption
+    constructor; assumption; assumption
+case _ j1 j2 j3 ih1 ih2 ih3 =>
+  apply Or.inr; apply Exists.intro ★
+  cases ih3; case _ ih3 => cases ih3
+  case _ ih3 =>
+  cases ih3; case _ K ih3 =>
+  cases ih3; case _ lem1 lem2 =>
+  cases lem2; case _ q1 q2 q3 =>
+  cases ih1; case _ ih1 =>
+    apply And.intro lem1
+    apply Judgment.eq ih1 j1 j2
+  case _ ih1 =>
+    cases ih1; case _ K ih1 =>
+      cases ih1.2
+      cases ih1.1
+case _ j1 j2 j3 j4 ih1 ih2 ih3 ih4 =>
+  apply Or.inr; apply Exists.intro ★
+  cases ih4; case _ ih4 => cases ih4
+  case _ ih4 =>
+  cases ih4; case _ K ih4 =>
+  cases ih4; case _ lem1 lem2 =>
+  cases lem2; case _ q1 q2 q3 =>
+    apply And.intro lem1
+    apply Judgment.eq j1 j2 j3
+case _ Γ K _ _ _ j1 j2 ih1 ih2  =>
+  apply Or.inr; apply Exists.intro ★
+  cases ih2; case _ ih2 => cases ih2
+  case _ ih2 =>
+  cases ih2; case _ K ih2 =>
+  cases ih2; case _ lem1 lem2 =>
+  cases lem2; case _ q1 q2 q3 =>
+    have wf : ⊢ Γ := by
+      have lem := judgment_ctx_wf j2
+      cases lem; assumption
+    have lem3 : Γ ⊢ ★ : □ := by
+      constructor; apply wf
+    apply And.intro lem3
+    apply Judgment.eq lem3
+    constructor; assumption; assumption
+    constructor; assumption; assumption
+case _ j1 j2 j3 j4 ih1 ih2 =>
+  apply Or.inr; apply Exists.intro ★
+  cases ih1; case _ ih1 => cases ih1
+  case _ ih1 =>
+  cases ih1; case _ K1 ih1 =>
+  cases ih1; case _ lem1 lem2 =>
+  cases lem2; case _ q1 q2 q3 =>
+  cases q2; case _ q2 q4 =>
+  cases q3; case _ q3 q5 =>
+  cases ih2; case _ ih2 => cases ih2
+  case _ ih2 =>
+  cases ih2; case _ K2 ih2 =>
+  cases ih2; case _ lem3 lem4 =>
+  cases lem4; case _ w1 w2 w3 =>
+    have lem5 := beta_kind q4 w2; simp at lem5
+    have lem6 := beta_kind q5 w3; simp at lem6
+    apply And.intro lem3
+    apply Judgment.eq lem3 lem5 lem6
+case _ h ih =>
+  apply Or.inr; apply Or.inr
+  apply Exists.intro .type; apply And.intro
+  constructor; apply judgment_ctx_wf h
+  apply h
 
 theorem kind_disjoint :
   Γ ⊢ t : A -> A = .kind ->
@@ -395,35 +427,3 @@ case _ =>
   cases h; case _ K h =>
   cases h; case _ h1 h2 =>
   cases h2
-
-theorem type_disjoint :
-  Γ ⊢ t : A -> Γ ⊢ A : .kind ->
-  ¬ (A = .kind) ∧ ¬ (∃ K, Γ ⊢ K : .kind ∧ Γ ⊢ A : K)
-:= by
-intro j1 j2
-apply And.intro
-case _ =>
-  intro h; subst h; cases j2
-case _ =>
-  intro h
-  cases h; case _ K h =>
-  cases h; case _ h1 h2 =>
-    have lem := uniqueness_of_types j2 h2; subst lem
-    cases h1
-
-theorem term_disjoint :
-  Γ ⊢ t : A -> (∃ K, Γ ⊢ K : .kind ∧ Γ ⊢ A : K) ->
-  ¬ (A = .kind) ∧ ¬ (Γ ⊢ A : .kind)
-:= by
-intro j1 j2
-have lem := classification_lemma j1; simp at lem
-cases j2; case _ K j2 =>
-cases j2; case _ j2 j2' =>
-  apply And.intro
-  case _ =>
-    intro h; subst h
-    cases j2'
-  case _ =>
-    intro h
-    have lem := uniqueness_of_types j2' h; subst lem
-    cases j2
