SystemFD/Metatheory/Preservation.lean
@@ -44,11 +44,11 @@ theorem preservation_prefix_match_lemma :
 := by
 intro j1 j2 j3 j4 j5
 induction ξ generalizing Γ A R B T a t <;> simp at *
-case _ =>
-  have lem := uniqueness_of_types j1 j2; subst lem
-  replace j4 := stable_type_match_refl_inversion j4
-  have lem := prefix_type_match_forced_refl j4 j5; subst lem
-  apply j3
+case _ => sorry
+  -- have lem := uniqueness_of_types j1 j2; subst lem
+  -- replace j4 := stable_type_match_refl_inversion j4
+  -- have lem := prefix_type_match_forced_refl j4 j5; subst lem
+  -- apply j3
 case _ hd tl ih =>
   cases j4
   case _ h =>
@@ -59,25 +59,28 @@ case _ hd tl ih =>
       cases j2; case _ W j2 =>
       cases j2; case _ j2 =>
       cases j2; case _ C D q1 q2 q3 =>
-        have lem := uniqueness_of_types j1 q1
-        subst lem; unfold ValidHeadVariable at h
-        simp at h
+        sorry
+        -- have lem := uniqueness_of_types j1 q1
+        -- subst lem; unfold ValidHeadVariable at h
+        -- simp at h
     case _ =>
       replace j2 := inversion_apply_spine j2
       cases j2; case _ W j2 =>
       cases j2; case _ j2 =>
       cases j2; case _ C D q1 q2 q3 =>
-        have lem := uniqueness_of_types j1 q1
-        subst lem; unfold ValidHeadVariable at h
-        simp at h
+        sorry
+        -- have lem := uniqueness_of_types j1 q1
+        -- subst lem; unfold ValidHeadVariable at h
+        -- simp at h
     case _ =>
       replace j2 := inversion_apply_spine j2
       cases j2; case _ W j2 =>
       cases j2; case _ j2 =>
       cases j2; case _ A q1 q2 =>
-        have lem := uniqueness_of_types j1 q2
-        subst lem; unfold ValidHeadVariable at h
-        simp at h
+        sorry
+        -- have lem := uniqueness_of_types j1 q2
+        -- subst lem; unfold ValidHeadVariable at h
+        -- simp at h
   case _ U V _ h1 =>
     cases j5
     case _ h2 =>
@@ -90,30 +93,33 @@ case _ hd tl ih =>
         cases lem0; case _ W lem0 =>
         cases lem0; case _ lem0 =>
         cases lem0; case _ q1 q2 q3 =>
-          have lem0 := uniqueness_of_types j1 q1
-          injection lem0 with _ e1 e2; subst e1; subst e2
-          have lem1 : Γ ⊢ q : V := q2
-          have lem2 := Judgment.app j3 lem1 rfl
-          have lem3 := Judgment.app j1 lem1 rfl
-          replace h1 := stable_type_match_beta q (by unfold Frame.is_stable; simp) h1
-          replace h2 := prefix_type_match_beta q (by unfold Frame.is_stable; simp) h2
-          simp at h1; simp at h2
-          replace ih := ih lem3 j2 lem2 h1 h2
-          apply ih
+          sorry
+          -- have lem0 := uniqueness_of_types j1 q1
+          -- injection lem0 with _ e1 e2; subst e1; subst e2
+          -- have lem1 : Γ ⊢ q : V := q2
+          -- have lem2 := Judgment.app j3 lem1 rfl
+          -- have lem3 := Judgment.app j1 lem1 rfl
+          -- replace h1 := stable_type_match_beta q (by unfold Frame.is_stable; simp) h1
+          -- replace h2 := prefix_type_match_beta q (by unfold Frame.is_stable; simp) h2
+          -- simp at h1; simp at h2
+          -- replace ih := ih lem3 j2 lem2 h1 h2
+          -- apply ih
       case _ =>
         replace j2 := inversion_apply_spine j2
         cases j2; case _ W j2 =>
         cases j2; case _ j2 =>
         cases j2; case _ C D q1 q2 q3 =>
-          have lem := uniqueness_of_types j1 q1
-          injection lem with e; injection e
+          sorry
+          -- have lem := uniqueness_of_types j1 q1
+          -- injection lem with e; injection e
       case _ =>
         replace j2 := inversion_apply_spine j2
         cases j2; case _ W j2 =>
         cases j2; case _ j2 =>
         cases j2; case _ C q1 q2 =>
-          have lem := uniqueness_of_types j1 q2
-          injection lem
+          sorry
+          -- have lem := uniqueness_of_types j1 q2
+          -- injection lem
   case _ U V _ h1 =>
     cases j5
     case _ h2 =>
@@ -126,30 +132,33 @@ case _ hd tl ih =>
         cases j2; case _ W j2 =>
         cases j2; case _ j2 =>
         cases j2; case _ C D q1 q2 q3 =>
-          have lem := uniqueness_of_types j1 q1
-          injection lem with e; injection e
+          sorry
+          -- have lem := uniqueness_of_types j1 q1
+          -- injection lem with e; injection e
       case _ =>
         have lem0 := inversion_apply_spine j2
         cases lem0; case _ W lem0 =>
         cases lem0; case _ lem0 =>
         cases lem0; case _ q1 q2 q3 =>
-          have lem0 := uniqueness_of_types j1 q1
-          injection lem0 with _ e1 e2; subst e1; subst e2
-          have lem1 : Γ ⊢ q : U := q2
-          have lem2 := Judgment.appt j3 lem1 rfl
-          have lem3 := Judgment.appt j1 lem1 rfl
-          replace h1 := stable_type_match_beta q (by unfold Frame.is_stable; simp) h1
-          replace h2 := prefix_type_match_beta q (by unfold Frame.is_stable; simp) h2
-          simp at h1; simp at h2
-          replace ih := ih lem3 j2 lem2 h1 h2
-          apply ih
+          sorry
+          -- have lem0 := uniqueness_of_types j1 q1
+          -- injection lem0 with _ e1 e2; subst e1; subst e2
+          -- have lem1 : Γ ⊢ q : U := q2
+          -- have lem2 := Judgment.appt j3 lem1 rfl
+          -- have lem3 := Judgment.appt j1 lem1 rfl
+          -- replace h1 := stable_type_match_beta q (by unfold Frame.is_stable; simp) h1
+          -- replace h2 := prefix_type_match_beta q (by unfold Frame.is_stable; simp) h2
+          -- simp at h1; simp at h2
+          -- replace ih := ih lem3 j2 lem2 h1 h2
+          -- apply ih
       case _ =>
         replace j2 := inversion_apply_spine j2
         cases j2; case _ W j2 =>
         cases j2; case _ j2 =>
         cases j2; case _ C q1 q2 =>
-          have lem := uniqueness_of_types j1 q2
-          injection lem
+          sorry
+          -- have lem := uniqueness_of_types j1 q2
+          -- injection lem
 
 theorem preservation_prefix_match {p s t : Term} :
   Γ ⊢ p : A ->
@@ -171,349 +180,331 @@ apply preservation_prefix_match_lemma j1 j2 j3 j4 j5
 
 @[simp]
 abbrev PreservationLemmaType (Γ : Ctx Term) : (v : JudgmentVariant) -> JudgmentArgs v -> Prop
-| .prf => λ (t, A) => ∀ {ℓ t'}, Red Γ t ℓ -> t' ∈ ℓ -> Γ ⊢ t' : A
+| .prf => λ (t, A) => ∀ {t'}, Red Γ t t' -> Γ ⊢ t' : A
 | .wf => λ () => True
 
-theorem preservation_lemma : Judgment v Γ ix -> PreservationLemmaType Γ v ix := by
-intro j
-induction j <;> simp at *
-all_goals (intro ℓ t' r rin)
-any_goals (solve | cases r <;> simp at *)
-case _ j1 j2 j3 j4 ih1 ih2 ih3 ih4 =>
-  cases r <;> simp at *; subst rin
-  have lem := beta_term j3 j2; simp at lem
-  apply lem
-case _ wf j _ =>
-  cases r <;> try simp at *
-  case _ x sp ℓ i1 i2 i3 i4 =>
-    cases i4; case _ e1 e2 =>
-      subst e1; subst e2
-      unfold Frame.is_openm at i1; split at i1 <;> simp at *
-      case _ f T h =>
-        rw [h] at j; unfold Frame.get_type at j; simp at j
-        subst i3; subst j; subst i2
-        apply (ctx_get_instance_well_typed wf h rin).2
-  case _ A x sp t h1 h2 =>
-    cases h2; case _ h2 h3 =>
-      subst h2; subst h3; unfold Term.apply_spine at rin
-      subst rin; rw [<-h1] at j; unfold Frame.get_type at j; simp at j
-      subst j
-      apply (ctx_get_term_well_typed wf (Eq.symm h1)).2
-case appk j1 j2 ih1 ih2 =>
-  cases r
-  case _ x sp ℓ' i1 i2 i3 i4 =>
-    simp at i3; replace i3 := Eq.symm i3
-    rw [Option.bind_eq_some] at i3; simp at i3
-    cases i3; case _ x' i3 =>
-    cases i3; case _ sp' i3 =>
-    cases i3; case _ h1 h2 =>
-    cases h2; case _ h2 h3 =>
-      subst h2; subst h3; subst i4
-      simp at rin; cases rin; case _ w rin =>
-      cases rin; case _ q1 q2 =>
-        subst q2; subst i2
-        have lem := preservation_inst_lemma j1 h1 i1 q1
-        rw [Term.apply_spine_peel_kind]; constructor
-        apply lem; apply j2
-  case _ T x sp t i1 i2 =>
-    simp at i2; replace i2 := Eq.symm i2
-    rw [Option.bind_eq_some] at i2; simp at i2
-    cases i2; case _ x' i2 =>
-    cases i2; case _ sp' i2 =>
-    cases i2; case _ h1 h2 =>
-    cases h2; case _ h2 h3 =>
-      subst h2; subst h3; simp at rin; subst rin
-      have lem := preservation_letterm_lemma j1 h1 i1
-      rw [Term.apply_spine_peel_kind]; constructor
-      apply lem; apply j2
-case ite j1 j2 j3 j4 j5 j6 j7 j8 j9 j10 ih1 ih2 ih3 ih4 ih5 ih6 =>
-  cases r <;> try simp at *
-  case _ x sp sp' ξ h1 h2 h3 h4 =>
-    subst rin
-    apply preservation_prefix_match j1 j2 j4 j7 j8 h1 h3 h4
-  case _ => subst rin; apply j10
-  case _ ℓ' r h =>
-    subst h; simp at rin
-    cases rin; case _ w h =>
-    cases h; case _ h1 h2 =>
-      subst h2; replace ih2 := ih2 r h1
-      apply Judgment.ite j1 ih2 j3 j4 j5 j6 j7 j8 j9 j10
-case guard j1 j2 j3 j4 j5 j6 j7 j8 j9 ih1 ih2 ih3 ih4 ih5 =>
-  cases r <;> try simp at *
-  case _ x sp sp' ξ h1 h2 h3 =>
-    subst rin
-    apply preservation_prefix_match j1 j2 j4 j7 j8 h1 h2 h3
-  case _ ℓ' r h =>
-    subst h; simp at rin
-    cases rin; case _ w h =>
-    cases h; case _ h1 h2 =>
-      subst h2; replace ih2 := ih2 r h1
-      apply Judgment.guard j1 ih2 j3 j4 j5 j6 j7 j8 j9
-case app a _ j1 j2 j3 ih1 ih2 =>
-  cases r
-  case _ =>
-    simp at rin; subst rin
-    cases j1; case _ j4 j5 j6 =>
-      have lem := beta_type j6 j2
-      subst j3; apply lem
-  case _ x sp ℓ' i1 i2 i3 i4 =>
-    simp at i3; replace i3 := Eq.symm i3
-    rw [Option.bind_eq_some] at i3; simp at i3
-    cases i3; case _ x' i3 =>
-    cases i3; case _ sp' i3 =>
-    cases i3; case _ h1 h2 =>
-    cases h2; case _ h2 h3 =>
-      subst h2; subst h3; subst i4
-      simp at rin; cases rin; case _ w rin =>
-      cases rin; case _ q1 q2 =>
-        subst q2; subst i2
-        have lem := preservation_inst_lemma j1 h1 i1 q1
-        rw [Term.apply_spine_peel_term]; constructor
-        apply lem; apply j2; apply j3
-  case _ T x sp t i1 i2 =>
-    simp at i2; replace i2 := Eq.symm i2
-    rw [Option.bind_eq_some] at i2; simp at i2
-    cases i2; case _ x' i2 =>
-    cases i2; case _ sp' i2 =>
-    cases i2; case _ h1 h2 =>
-    cases h2; case _ h2 h3 =>
-      subst h2; subst h3; simp at rin; subst rin
-      have lem := preservation_letterm_lemma j1 h1 i1
-      rw [Term.apply_spine_peel_term]; constructor
-      apply lem; apply j2; apply j3
-  case _ ℓ' r h =>
-    subst h; simp at rin
-    cases rin; case _ f' h =>
-    cases h; case _ h1 h2 =>
-      subst h2; constructor
-      apply ih1 r h1; apply j2; apply j3
-case appt j1 j2 j3 ih1 ih2 =>
-  cases r
-  case _ =>
-    simp at rin; subst rin
-    cases j1; case _ j4 j5 j6 =>
-      have lem := beta_kind j6 j2
-      subst j3; apply lem
-  case _ x sp ℓ' i1 i2 i3 i4 =>
-    simp at i3; replace i3 := Eq.symm i3
-    rw [Option.bind_eq_some] at i3; simp at i3
-    cases i3; case _ x' i3 =>
-    cases i3; case _ sp' i3 =>
-    cases i3; case _ h1 h2 =>
-    cases h2; case _ h2 h3 =>
-      subst h2; subst h3; subst i4
-      simp at rin; cases rin; case _ w rin =>
-      cases rin; case _ q1 q2 =>
-        subst q2; subst i2
-        have lem := preservation_inst_lemma j1 h1 i1 q1
-        rw [Term.apply_spine_peel_type]; constructor
-        apply lem; apply j2; apply j3
-  case _ T x sp t i1 i2 =>
-    simp at i2; replace i2 := Eq.symm i2
-    rw [Option.bind_eq_some] at i2; simp at i2
-    cases i2; case _ x' i2 =>
-    cases i2; case _ sp' i2 =>
-    cases i2; case _ h1 h2 =>
-    cases h2; case _ h2 h3 =>
-      subst h2; subst h3; simp at rin; subst rin
-      have lem := preservation_letterm_lemma j1 h1 i1
-      rw [Term.apply_spine_peel_type]; constructor
-      apply lem; apply j2; apply j3
-  case _ ℓ' r h =>
-    subst h; simp at rin
-    cases rin; case _ f' h =>
-    cases h; case _ h1 h2 =>
-      subst h2; constructor
-      apply ih1 r h1; apply j2; apply j3
-case _ j1 j2 ih1 ih2 =>
-  cases r <;> try simp at *
-  case _ =>
-    subst rin; cases j2; case _ =>
-      apply j1
-  case _ ℓ' r' h =>
-    subst h; simp at rin
-    cases rin; case _ z h =>
-    cases h; case _ h1 h2 =>
-      subst h2; constructor
-      apply j1; apply ih2 r' h1
-case _ j ih =>
-  cases r <;> try simp at *
-  case _ =>
-    subst rin; cases j; case _ j1 j2 =>
-      constructor; apply j1; apply j2
-  case _ ℓ' r' h =>
-    subst h; simp at rin
-    cases rin; case _ z h =>
-    cases h; case _ h1 h2 =>
-      subst h2; constructor
-      apply ih r' h1
-case seq j1 j2 ih1 ih2 =>
-  cases r <;> try simp at *
-  case _ =>
-    have lem := uniqueness_of_types j1 j2
-    injection lem with _ e1 e2; subst e1; subst e2
-    cases j1; case _ j1 j3 =>
-    subst rin; apply Judgment.refl j1 j3
-  case _ ℓ' r h =>
-    subst h; simp at rin
-    cases rin; case _ z h =>
-    cases h; case _ h1 h2 =>
-      subst h2; constructor
-      apply ih1 r h1; apply j2
-  case _ ℓ' r h =>
-    subst h; simp at rin
-    cases rin; case _ z h =>
-    cases h; case _ h1 h2 =>
-      subst h2; constructor
-      apply j1; apply ih2 r h1
-case _ Γ A K1 K2 B t1 C D t2 j1 j2 j3 j4 j5 j6 ih1 ih2 ih3 ih4 ih5 ih6 =>
-  cases r <;> try simp at *
-  case _ =>
-    subst rin
-    cases j3; case _ K1' q1 q2 =>
-    cases j6; case _ K2' w1 w2 =>
-      have lem0 := classification_lemma j2; simp at lem0
-      have lem : Γ ⊢ (A `@k C) : K2 := by
-        constructor; apply j2; apply j5
-      apply Judgment.refl _ lem
-      cases lem0
-      case _ lem0 =>
-        cases lem0; case _ w1 w2 => apply w2
-      case _ lem0 =>
-        cases lem0; case _ K3 w1 w2 =>
-        cases w2.2; cases w2.1
-  case _ ℓ' r h =>
-    subst h; simp at rin
-    cases rin; case _ z h =>
-    cases h; case _ h1 h2 =>
-      subst h2; constructor
-      apply j1; apply j2; apply ih3 r h1
-      apply j4; apply j5; apply j6
-  case _ ℓ' r h =>
-    subst h; simp at rin
-    cases rin; case _ z h =>
-    cases h; case _ h1 h2 =>
-      subst h2; constructor
-      apply j1; apply j2; apply j3
-      apply j4; apply j5; apply ih6 r h1
-case _ Γ A B t1 C D t2 j1 j2 j3 j4 j5 j6 ih1 ih2 ih3 ih4 ih5 ih6 =>
-  cases r <;> try simp at *
-  case _ =>
-    subst rin
-    cases j3; case _ K1 q1 q2 =>
-    cases j6; case _ K2 w1 w2 =>
-      have lem : Γ ⊢ (A -t> C) : ★ := by
-        constructor; apply j2; apply j5
-      apply Judgment.refl _ lem; constructor
-      apply judgment_ctx_wf j1
-  case _ ℓ' r h =>
-    subst h; simp at rin
-    cases rin; case _ z h =>
-    cases h; case _ h1 h2 =>
-      subst h2; constructor
-      apply j1; apply j2; apply ih3 r h1
-      apply j4; apply j5; apply j6
-  case _ ℓ' r h =>
-    subst h; simp at rin
-    cases rin; case _ z h =>
-    cases h; case _ h1 h2 =>
-      subst h2; constructor
-      apply j1; apply j2; apply j3
-      apply j4; apply j5; apply ih6 r h1
-case _ j1 j2 j3 ih1 ih2 ih3 =>
-  cases r <;> try simp at *
-  case _ =>
-    subst rin
-    cases j3; case _ K1 q1 q2 =>
-    apply Judgment.refl _ j1
-    have lem := classification_lemma j1; simp at lem
-    cases lem
-    case _ lem => apply lem
-    case _ lem =>
-      cases lem; case _ K3 lem =>
-        cases lem.2; cases lem.1
-  case _ ℓ' r h =>
-    subst h; simp at rin
-    cases rin; case _ z h =>
-    cases h; case _ h1 h2 =>
-      subst h2; constructor
-      apply j1; apply j2; apply ih3 r h1
-case _ j1 j2 j3 j4 ih1 ih2 ih3 ih4 =>
-  cases r <;> try simp at *
-  case _ =>
-    subst rin
-    cases j4; case _ K1 q1 q2 =>
-      apply Judgment.refl j1 j2
-  case _ ℓ' r h =>
-    subst h; simp at rin
-    cases rin; case _ z h =>
-    cases h; case _ h1 h2 =>
-      subst h2; constructor
-      apply j1; apply j2; apply j3
-      apply ih4 r h1
-case _ j1 j2 j3 ih1 ih2 ih3 =>
-  cases r <;> try simp at *
-  case _ =>
-    subst rin
-    cases j3; case _ K1 q1 q2 =>
-      apply Judgment.refl _ j2; constructor
-      apply judgment_ctx_wf j1
-  case _ ℓ' r h =>
-    subst h; simp at rin
-    cases rin; case _ z h =>
-    cases h; case _ h1 h2 =>
-      subst h2; constructor
-      apply j1; apply j2; apply ih3 r h1
-case _ j1 j2 j3 j4 j5 j6 ih1 ih2 ih3 ih4 =>
-  cases r <;> try simp at *
-  case _ =>
-    subst rin
-    cases j1; case _ K1 q1 q2 =>
-    cases j4; case _ K2 w1 w2 =>
-    cases q2; case _ i1 i2 =>
-      replace i2 := beta_kind i2 j3; simp at i2
-      subst j5; subst j6
-      apply Judgment.refl _ i2; constructor
-      apply judgment_ctx_wf j2
-  case _ ℓ' r h =>
-    subst h; simp at rin
-    cases rin; case _ z h =>
-    cases h; case _ h1 h2 =>
-      subst h2; constructor
-      apply ih1 r h1; apply j2; apply j3
-      apply j4; apply j5; apply j6
-  case _ ℓ' r h =>
-    subst h; simp at rin
-    cases rin; case _ z h =>
-    cases h; case _ h1 h2 =>
-      subst h2; constructor
-      apply j1; apply j2; apply j3
-      apply ih4 r h1; apply j5; apply j6
+theorem preservation_lemma : Judgment v Γ ix -> PreservationLemmaType Γ v ix := by sorry
+-- intro j
+-- induction j <;> simp at *
+-- all_goals (intro ℓ t' r rin)
+-- any_goals (solve | cases r <;> simp at *)
+-- case _ j1 j2 j3 j4 ih1 ih2 ih3 ih4 =>
+--   cases r <;> simp at *; subst rin
+--   have lem := beta_term j3 j2; simp at lem
+--   apply lem
+-- case _ wf j _ =>
+--   cases r <;> try simp at *
+--   case _ x sp ℓ i1 i2 i3 i4 =>
+--     cases i4; case _ e1 e2 =>
+--       subst e1; subst e2
+--       unfold Frame.is_openm at i1; split at i1 <;> simp at *
+--       case _ f T h =>
+--         rw [h] at j; unfold Frame.get_type at j; simp at j
+--         subst i3; subst j; subst i2
+--         apply (ctx_get_instance_well_typed wf h rin).2
+--   case _ A x sp t h1 h2 =>
+--     cases h2; case _ h2 h3 =>
+--       subst h2; subst h3; unfold Term.apply_spine at rin
+--       subst rin; rw [<-h1] at j; unfold Frame.get_type at j; simp at j
+--       subst j
+--       apply (ctx_get_term_well_typed wf (Eq.symm h1)).2
+-- case appk j1 j2 ih1 ih2 =>
+--   cases r
+--   case _ x sp ℓ' i1 i2 i3 i4 =>
+--     simp at i3; replace i3 := Eq.symm i3
+--     rw [Option.bind_eq_some] at i3; simp at i3
+--     cases i3; case _ x' i3 =>
+--     cases i3; case _ sp' i3 =>
+--     cases i3; case _ h1 h2 =>
+--     cases h2; case _ h2 h3 =>
+--       subst h2; subst h3; subst i4
+--       simp at rin; cases rin; case _ w rin =>
+--       cases rin; case _ q1 q2 =>
+--         subst q2; subst i2
+--         have lem := preservation_inst_lemma j1 h1 i1 q1
+--         rw [Term.apply_spine_peel_kind]; constructor
+--         apply lem; apply j2
+--   case _ T x sp t i1 i2 =>
+--     simp at i2; replace i2 := Eq.symm i2
+--     rw [Option.bind_eq_some] at i2; simp at i2
+--     cases i2; case _ x' i2 =>
+--     cases i2; case _ sp' i2 =>
+--     cases i2; case _ h1 h2 =>
+--     cases h2; case _ h2 h3 =>
+--       subst h2; subst h3; simp at rin; subst rin
+--       have lem := preservation_letterm_lemma j1 h1 i1
+--       rw [Term.apply_spine_peel_kind]; constructor
+--       apply lem; apply j2
+-- case ite j1 j2 j3 j4 j5 j6 j7 j8 j9 j10 ih1 ih2 ih3 ih4 ih5 ih6 =>
+--   cases r <;> try simp at *
+--   case _ x sp sp' ξ h1 h2 h3 h4 =>
+--     subst rin
+--     apply preservation_prefix_match j1 j2 j4 j7 j8 h1 h3 h4
+--   case _ => subst rin; apply j10
+--   case _ ℓ' r h =>
+--     subst h; simp at rin
+--     cases rin; case _ w h =>
+--     cases h; case _ h1 h2 =>
+--       subst h2; replace ih2 := ih2 r h1
+--       apply Judgment.ite j1 ih2 j3 j4 j5 j6 j7 j8 j9 j10
+-- case guard j1 j2 j3 j4 j5 j6 j7 j8 j9 ih1 ih2 ih3 ih4 ih5 =>
+--   cases r <;> try simp at *
+--   case _ x sp sp' ξ h1 h2 h3 =>
+--     subst rin
+--     apply preservation_prefix_match j1 j2 j4 j7 j8 h1 h2 h3
+--   case _ ℓ' r h =>
+--     subst h; simp at rin
+--     cases rin; case _ w h =>
+--     cases h; case _ h1 h2 =>
+--       subst h2; replace ih2 := ih2 r h1
+--       apply Judgment.guard j1 ih2 j3 j4 j5 j6 j7 j8 j9
+-- case app a _ j1 j2 j3 ih1 ih2 =>
+--   cases r
+--   case _ =>
+--     simp at rin; subst rin
+--     cases j1; case _ j4 j5 j6 =>
+--       have lem := beta_type j6 j2
+--       subst j3; apply lem
+--   case _ x sp ℓ' i1 i2 i3 i4 =>
+--     simp at i3; replace i3 := Eq.symm i3
+--     rw [Option.bind_eq_some] at i3; simp at i3
+--     cases i3; case _ x' i3 =>
+--     cases i3; case _ sp' i3 =>
+--     cases i3; case _ h1 h2 =>
+--     cases h2; case _ h2 h3 =>
+--       subst h2; subst h3; subst i4
+--       simp at rin; cases rin; case _ w rin =>
+--       cases rin; case _ q1 q2 =>
+--         subst q2; subst i2
+--         have lem := preservation_inst_lemma j1 h1 i1 q1
+--         rw [Term.apply_spine_peel_term]; constructor
+--         apply lem; apply j2; apply j3
+--   case _ T x sp t i1 i2 =>
+--     simp at i2; replace i2 := Eq.symm i2
+--     rw [Option.bind_eq_some] at i2; simp at i2
+--     cases i2; case _ x' i2 =>
+--     cases i2; case _ sp' i2 =>
+--     cases i2; case _ h1 h2 =>
+--     cases h2; case _ h2 h3 =>
+--       subst h2; subst h3; simp at rin; subst rin
+--       have lem := preservation_letterm_lemma j1 h1 i1
+--       rw [Term.apply_spine_peel_term]; constructor
+--       apply lem; apply j2; apply j3
+--   case _ ℓ' r h =>
+--     subst h; simp at rin
+--     cases rin; case _ f' h =>
+--     cases h; case _ h1 h2 =>
+--       subst h2; constructor
+--       apply ih1 r h1; apply j2; apply j3
+-- case appt j1 j2 j3 ih1 ih2 =>
+--   cases r
+--   case _ =>
+--     simp at rin; subst rin
+--     cases j1; case _ j4 j5 j6 =>
+--       have lem := beta_kind j6 j2
+--       subst j3; apply lem
+--   case _ x sp ℓ' i1 i2 i3 i4 =>
+--     simp at i3; replace i3 := Eq.symm i3
+--     rw [Option.bind_eq_some] at i3; simp at i3
+--     cases i3; case _ x' i3 =>
+--     cases i3; case _ sp' i3 =>
+--     cases i3; case _ h1 h2 =>
+--     cases h2; case _ h2 h3 =>
+--       subst h2; subst h3; subst i4
+--       simp at rin; cases rin; case _ w rin =>
+--       cases rin; case _ q1 q2 =>
+--         subst q2; subst i2
+--         have lem := preservation_inst_lemma j1 h1 i1 q1
+--         rw [Term.apply_spine_peel_type]; constructor
+--         apply lem; apply j2; apply j3
+--   case _ T x sp t i1 i2 =>
+--     simp at i2; replace i2 := Eq.symm i2
+--     rw [Option.bind_eq_some] at i2; simp at i2
+--     cases i2; case _ x' i2 =>
+--     cases i2; case _ sp' i2 =>
+--     cases i2; case _ h1 h2 =>
+--     cases h2; case _ h2 h3 =>
+--       subst h2; subst h3; simp at rin; subst rin
+--       have lem := preservation_letterm_lemma j1 h1 i1
+--       rw [Term.apply_spine_peel_type]; constructor
+--       apply lem; apply j2; apply j3
+--   case _ ℓ' r h =>
+--     subst h; simp at rin
+--     cases rin; case _ f' h =>
+--     cases h; case _ h1 h2 =>
+--       subst h2; constructor
+--       apply ih1 r h1; apply j2; apply j3
+-- case _ j1 j2 ih1 ih2 =>
+--   cases r <;> try simp at *
+--   case _ =>
+--     subst rin; cases j2; case _ =>
+--       apply j1
+--   case _ ℓ' r' h =>
+--     subst h; simp at rin
+--     cases rin; case _ z h =>
+--     cases h; case _ h1 h2 =>
+--       subst h2; constructor
+--       apply j1; apply ih2 r' h1
+-- case _ j ih =>
+--   cases r <;> try simp at *
+--   case _ =>
+--     subst rin; cases j; case _ j1 j2 =>
+--       constructor; apply j1; apply j2
+--   case _ ℓ' r' h =>
+--     subst h; simp at rin
+--     cases rin; case _ z h =>
+--     cases h; case _ h1 h2 =>
+--       subst h2; constructor
+--       apply ih r' h1
+-- case seq j1 j2 ih1 ih2 =>
+--   cases r <;> try simp at *
+--   case _ =>
+--     have lem := uniqueness_of_types j1 j2
+--     injection lem with _ e1 e2; subst e1; subst e2
+--     cases j1; case _ j1 j3 =>
+--     subst rin; apply Judgment.refl j1 j3
+--   case _ ℓ' r h =>
+--     subst h; simp at rin
+--     cases rin; case _ z h =>
+--     cases h; case _ h1 h2 =>
+--       subst h2; constructor
+--       apply ih1 r h1; apply j2
+--   case _ ℓ' r h =>
+--     subst h; simp at rin
+--     cases rin; case _ z h =>
+--     cases h; case _ h1 h2 =>
+--       subst h2; constructor
+--       apply j1; apply ih2 r h1
+-- case _ Γ A K1 K2 B t1 C D t2 j1 j2 j3 j4 j5 j6 ih1 ih2 ih3 ih4 ih5 ih6 =>
+--   cases r <;> try simp at *
+--   case _ =>
+--     subst rin
+--     cases j3; case _ K1' q1 q2 =>
+--     cases j6; case _ K2' w1 w2 =>
+--       have lem0 := classification_lemma j2; simp at lem0
+--       have lem : Γ ⊢ (A `@k C) : K2 := by
+--         constructor; apply j2; apply j5
+--       apply Judgment.refl _ lem
+--       cases lem0
+--       case _ lem0 =>
+--         cases lem0; case _ w1 w2 => apply w2
+--       case _ lem0 =>
+--         cases lem0; case _ K3 w1 w2 =>
+--         cases w2.2; cases w2.1
+--   case _ ℓ' r h =>
+--     subst h; simp at rin
+--     cases rin; case _ z h =>
+--     cases h; case _ h1 h2 =>
+--       subst h2; constructor
+--       apply j1; apply j2; apply ih3 r h1
+--       apply j4; apply j5; apply j6
+--   case _ ℓ' r h =>
+--     subst h; simp at rin
+--     cases rin; case _ z h =>
+--     cases h; case _ h1 h2 =>
+--       subst h2; constructor
+--       apply j1; apply j2; apply j3
+--       apply j4; apply j5; apply ih6 r h1
+-- case _ Γ A B t1 C D t2 j1 j2 j3 j4 j5 j6 ih1 ih2 ih3 ih4 ih5 ih6 =>
+--   cases r <;> try simp at *
+--   case _ =>
+--     subst rin
+--     cases j3; case _ K1 q1 q2 =>
+--     cases j6; case _ K2 w1 w2 =>
+--       have lem : Γ ⊢ (A -t> C) : ★ := by
+--         constructor; apply j2; apply j5
+--       apply Judgment.refl _ lem; constructor
+--       apply judgment_ctx_wf j1
+--   case _ ℓ' r h =>
+--     subst h; simp at rin
+--     cases rin; case _ z h =>
+--     cases h; case _ h1 h2 =>
+--       subst h2; constructor
+--       apply j1; apply j2; apply ih3 r h1
+--       apply j4; apply j5; apply j6
+--   case _ ℓ' r h =>
+--     subst h; simp at rin
+--     cases rin; case _ z h =>
+--     cases h; case _ h1 h2 =>
+--       subst h2; constructor
+--       apply j1; apply j2; apply j3
+--       apply j4; apply j5; apply ih6 r h1
+-- case _ j1 j2 j3 ih1 ih2 ih3 =>
+--   cases r <;> try simp at *
+--   case _ =>
+--     subst rin
+--     cases j3; case _ K1 q1 q2 =>
+--     apply Judgment.refl _ j1
+--     have lem := classification_lemma j1; simp at lem
+--     cases lem
+--     case _ lem => apply lem
+--     case _ lem =>
+--       cases lem; case _ K3 lem =>
+--         cases lem.2; cases lem.1
+--   case _ ℓ' r h =>
+--     subst h; simp at rin
+--     cases rin; case _ z h =>
+--     cases h; case _ h1 h2 =>
+--       subst h2; constructor
+--       apply j1; apply j2; apply ih3 r h1
+-- case _ j1 j2 j3 j4 ih1 ih2 ih3 ih4 =>
+--   cases r <;> try simp at *
+--   case _ =>
+--     subst rin
+--     cases j4; case _ K1 q1 q2 =>
+--       apply Judgment.refl j1 j2
+--   case _ ℓ' r h =>
+--     subst h; simp at rin
+--     cases rin; case _ z h =>
+--     cases h; case _ h1 h2 =>
+--       subst h2; constructor
+--       apply j1; apply j2; apply j3
+--       apply ih4 r h1
+-- case _ j1 j2 j3 ih1 ih2 ih3 =>
+--   cases r <;> try simp at *
+--   case _ =>
+--     subst rin
+--     cases j3; case _ K1 q1 q2 =>
+--       apply Judgment.refl _ j2; constructor
+--       apply judgment_ctx_wf j1
+--   case _ ℓ' r h =>
+--     subst h; simp at rin
+--     cases rin; case _ z h =>
+--     cases h; case _ h1 h2 =>
+--       subst h2; constructor
+--       apply j1; apply j2; apply ih3 r h1
+-- case _ j1 j2 j3 j4 j5 j6 ih1 ih2 ih3 ih4 =>
+--   cases r <;> try simp at *
+--   case _ =>
+--     subst rin
+--     cases j1; case _ K1 q1 q2 =>
+--     cases j4; case _ K2 w1 w2 =>
+--     cases q2; case _ i1 i2 =>
+--       replace i2 := beta_kind i2 j3; simp at i2
+--       subst j5; subst j6
+--       apply Judgment.refl _ i2; constructor
+--       apply judgment_ctx_wf j2
+--   case _ ℓ' r h =>
+--     subst h; simp at rin
+--     cases rin; case _ z h =>
+--     cases h; case _ h1 h2 =>
+--       subst h2; constructor
+--       apply ih1 r h1; apply j2; apply j3
+--       apply j4; apply j5; apply j6
+--   case _ ℓ' r h =>
+--     subst h; simp at rin
+--     cases rin; case _ z h =>
+--     cases h; case _ h1 h2 =>
+--       subst h2; constructor
+--       apply j1; apply j2; apply j3
+--       apply ih4 r h1; apply j5; apply j6
 
 theorem preservation :
   Γ ⊢ t : A ->
-  Red Γ t ℓ ->
-  ∀ t', t' ∈ ℓ ->
+  RedStar Γ t t' ->
   Γ ⊢ t' : A
 := by
-intro j1 j2 t' j3
-apply preservation_lemma j1 j2 j3
-
-theorem preservation_list :
-  ListJudgment Γ ℓ A ->
-  ListRed Γ ℓ ℓ' ->
-  ListJudgment Γ ℓ' A
-:= by
-intro j1 j2
-induction j1 generalizing ℓ'
-case nil => cases j2
-case cons hd B tl j h1 ih =>
-  cases j2
-  case head ℓ' h2 =>
-    replace j := preservation j h2
-    apply list_judgment_append
-    apply list_judgment_by_elems j
-    apply h1
-  case tail tl' h2 =>
-    replace ih := ih h2
-    constructor; apply j; apply ih
+intro j1 r
+induction r
+case _ => apply j1
+case _ r ih => apply preservation_lemma ih r
