SystemFD/Reduction.lean
@@ -2,22 +2,64 @@ import SystemFD.Util
 import SystemFD.Term
 import SystemFD.Ctx
 
-inductive Red : Ctx Term -> Term -> List Term -> Prop where
+def ctor2_has_congr1 : Ctor2Variant -> Bool
+| .refl => false
+| .arrowk => false
+| .appk => false
+| .appt => true
+| .app => true
+| .cast => false
+| .seq => true
+| .appc => true
+| .apptc => true
+| .choice => true
+
+def ctor2_has_congr2 : Ctor2Variant -> Bool
+| .refl => false
+| .arrowk => false
+| .appk => false
+| .appt => false
+| .app => false
+| .cast => true
+| .seq => true
+| .appc => true
+| .apptc => true
+| .choice => true
+
+def bind2_has_congr1 : Bind2Variant -> Bool
+| .all => false
+| .lamt => false
+| .lam => false
+| .arrow => false
+| .allc => false
+| .arrowc => true
+
+def bind2_has_congr2 : Bind2Variant -> Bool
+| .all => false
+| .lamt => false
+| .lam => false
+| .arrow => false
+| .allc => true
+| .arrowc => true
+
+inductive Red : Ctx Term -> Term -> Term -> Prop where
 ----------------------------------------------------------------
 ---- Basic Reduction Steps
 ----------------------------------------------------------------
-| beta : Red Γ ((`λ[A] b) `@ t) [b β[t]]
-| betat : Red Γ ((Λ[A] b) `@t t) [b β[t]]
-| letbeta : Red Γ (.letterm A t b) [b β[t]]
-| cast : Red Γ (t ▹ refl! A) [t]
-| sym : Red Γ (sym! (refl! A)) [refl! A]
-| seq : Red Γ ((refl! A) `; (refl! A)) [refl! A]
-| appc : Red Γ (refl! A `@c (refl! B)) [refl! (A `@k B)]
-| apptc : Red Γ (refl! (∀[K] A) `@c[refl! B]) [refl! (A β[B])]
-| fst : Red Γ (.ctor1 .fst (refl! (A `@k B))) [refl! A]
-| snd : Red Γ (.ctor1 .snd (refl! (A `@k B))) [refl! B]
-| allc : Red Γ (∀c[A] refl! B) [refl! (∀[A] B)]
-| arrowc : Red Γ (refl! A -c> refl! B) [refl! (A -t> B)]
+| beta : Red Γ ((`λ[A] b) `@ t) (b β[t])
+| betat : Red Γ ((Λ[A] b) `@t t) (b β[t])
+| letbeta : Red Γ (.letterm A t b) (b β[t])
+| cast : Red Γ (t ▹ refl! K A) t
+| sym : Red Γ (sym! (refl! K A)) (refl! K A)
+| seq : Red Γ ((refl! K A) `; (refl! K A)) (refl! K A)
+| appc : Red Γ (refl! K A `@c (refl! K B)) (refl! K (A `@k B))
+| apptc : Red Γ (refl! K (∀[K] A) `@c[refl! K B]) (refl! K (A β[B]))
+| fst : Red Γ (.ctor1 .fst (refl! K (A `@k B))) (refl! K A)
+| snd : Red Γ (.ctor1 .snd (refl! K (A `@k B))) (refl! K B)
+| allc : Red Γ (∀c[A] refl! K B) (refl! K (∀[A] B))
+| arrowc : Red Γ (refl! K A -c> refl! K B) (refl! K (A -t> B))
+| choice1 : Red Γ (`0 ⊕ t) t
+| choice2 : Red Γ (t ⊕ `0) t
 ----------------------------------------------------------------
 ---- Ite Matching
 ----------------------------------------------------------------
@@ -26,13 +68,13 @@ inductive Red : Ctx Term -> Term -> List Term -> Prop where
   .some (x, sp') = Term.neutral_form s ->
   .some q = prefix_equal sp sp' ->
   Γ.is_ctor x ->
-  Red Γ (.ite p s b e) [b.apply_spine q]
+  Red Γ (.ite p s b e) (b.apply_spine q)
 | ite_missed :
   .some (x, sp) = Term.neutral_form p ->
   .some (x', sp') = Term.neutral_form s ->
   Γ.is_stable_red x' ->
   x ≠ x' ∨ prefix_equal sp sp' = .none ->
-  Red Γ (.ite p s b e) [e]
+  Red Γ (.ite p s b e) e
 ----------------------------------------------------------------
 ---- Guard Matching
 ----------------------------------------------------------------
@@ -40,13 +82,13 @@ inductive Red : Ctx Term -> Term -> List Term -> Prop where
   .some (x, sp) = Term.neutral_form p ->
   .some (x, sp') = Term.neutral_form s ->
   .some q = prefix_equal sp sp' ->
-  Red Γ (.guard p s b) [b.apply_spine q]
+  Red Γ (.guard p s b) (b.apply_spine q)
 | guard_missed :
   .some (x, sp) = Term.neutral_form p ->
   .some (x', sp') = Term.neutral_form s ->
   Γ.is_stable_red x' ->
   x ≠ x' ∨ prefix_equal sp sp' = .none ->
-  Red Γ (.guard p s b) []
+  Red Γ (.guard p s b) `0
 ----------------------------------------------------------------
 ---- Instance Instantiation
 ----------------------------------------------------------------
@@ -55,95 +97,86 @@ inductive Red : Ctx Term -> Term -> List Term -> Prop where
   Γ.is_openm x ->
   tl = get_instances Γ x ->
   tl' = List.map (λ x => x.apply_spine sp) tl ->
-  Red Γ h tl'
+  h' = List.foldl (·⊕·) `0 tl' ->
+  Red Γ h h'
 ----------------------------------------------------------------
 ---- Local Let Substitution
 ----------------------------------------------------------------
 | letterm :
   .some (x, sp) = Term.neutral_form h ->
   .term _ t = Γ d@ x ->
-  Red Γ h [t.apply_spine sp]
+  Red Γ h (t.apply_spine sp)
 ----------------------------------------------------------------
----- Contextual/Congruence Rules
+---- Congruence Rules
 ----------------------------------------------------------------
--- | apphead_congr :
---   .some (x, sp) = Term.neutral_form t ->
---   Red Γ (#x) t' ->
---   tl' = List.map (λ x => x.apply_spine sp) t' ->
---   Red Γ t tl'
-| app_congr :
-  Red Γ f tl ->
-  tl' = List.map (λ x => x `@ a) tl ->
-  Red Γ (f `@ a) tl'
-| appt_congr :
-  Red Γ f tl ->
-  tl' = List.map (λ x => x `@t a) tl ->
-  Red Γ (f `@t a) tl'
-| cast_congr :
-  Red Γ e tl ->
-  tl' = List.map (λ x => t ▹ x) tl ->
-  Red Γ (t ▹ e) tl'
+| ctor1_congr :
+  Red Γ t t' ->
+  Red Γ (.ctor1 v t) (.ctor1 v t')
+| ctor2_congr1 :
+  ctor2_has_congr1 v ->
+  Red Γ t1 t1' ->
+  Red Γ (.ctor2 v t1 t2) (.ctor2 v t1' t2)
+| ctor2_congr2 :
+  ctor2_has_congr2 v ->
+  Red Γ t2 t2' ->
+  Red Γ (.ctor2 v t1 t2) (.ctor2 v t1 t2')
+| bind2_congr1 :
+  bind2_has_congr1 v ->
+  Red Γ t1 t1' ->
+  Red Γ (.bind2 v t1 t2) (.bind2 v t1' t2)
+| bind2_congr2 :
+  bind2_has_congr2 v ->
+  Red Γ t2 t2' ->
+  Red Γ (.bind2 v t1 t2) (.bind2 v t1 t2')
 | ite_congr :
-  Red Γ s tl ->
-  tl' = List.map (λ x => .ite p x b e) tl ->
-  Red Γ (.ite p s b e) tl'
-| sym_congr :
-  Red Γ e tl ->
-  tl' = List.map (λ x => sym! x) tl ->
-  Red Γ (sym! e) tl'
-| seq_congr1 :
-  Red Γ u tl ->
-  tl' = List.map (λ x => x `; v) tl ->
-  Red Γ (u `; v) tl'
-| seq_congr2 :
-  Red Γ v tl ->
-  tl' = List.map (λ x => u `; x) tl ->
-  Red Γ (u `; v) tl'
-| arrowc_congr1 :
-  Red Γ u tl ->
-  tl' = List.map (λ x => x -c> v) tl ->
-  Red Γ (u -c> v) tl'
-| arrowc_congr2 :
-  Red (.empty :: Γ) v tl ->
-  tl' = List.map (λ x => u -c> x) tl ->
-  Red Γ (u -c> v) tl'
-| appc_congr1 :
-  Red Γ f tl ->
-  tl' = List.map (λ x => x `@c a) tl ->
-  Red Γ (f `@c a) tl'
-| appc_congr2 :
-  Red Γ a tl ->
-  tl' = List.map (λ x => f `@c x) tl ->
-  Red Γ (f `@c a) tl'
-| fst_congr :
-  Red Γ u tl ->
-  tl' = List.map (λ x => .ctor1 .fst x) tl ->
-  Red Γ (.ctor1 .fst u) tl'
-| snd_congr :
-  Red Γ u tl ->
-  tl' = List.map (λ x => .ctor1 .snd x) tl ->
-  Red Γ (.ctor1 .snd u) tl'
-| apptc_congr1 :
-  Red Γ f tl ->
-  tl' = List.map (λ x => x `@c[a]) tl ->
-  Red Γ (f `@c[a]) tl'
-| apptc_congr2 :
-  Red Γ a tl ->
-  tl' = List.map (λ x => f `@c[x]) tl ->
-  Red Γ (f `@c[a]) tl'
-| allc_congr :
-  Red (.kind A ::Γ) e tl ->
-  tl' = List.map (λ x => ∀c[A] x) tl ->
-  Red Γ (∀c[A] e) tl'
+  Red Γ s s' ->
+  Red Γ (.ite p s b e) (.ite p s' b e)
 | guard_congr :
-  Red Γ s tl ->
-  tl' = List.map (λ x => .guard p x b) tl ->
-  Red Γ (.guard p s b) tl'
+  Red Γ s s' ->
+  Red Γ (.guard p s b) (.guard p s' b)
+----------------------------------------------------------------
+---- Absorption Rules
+----------------------------------------------------------------
+| ctor1_absorb :
+  Red Γ (.ctor1 v `0) `0
+| ctor2_abosrb1 :
+  ctor2_has_congr1 v ->
+  Red Γ (.ctor2 v `0 t2) `0
+| ctor2_abosrb2 :
+  ctor2_has_congr2 v ->
+  Red Γ (.ctor2 v t1 `0) `0
+| bind2_abosrb1 :
+  bind2_has_congr1 v ->
+  Red Γ (.bind2 v `0 t2) `0
+| bind2_abosrb2 :
+  bind2_has_congr2 v ->
+  Red Γ (.bind2 v t1 `0) `0
+| ite_abosrb :
+  Red Γ (.ite p `0 b e) `0
+| guard_abosrb :
+  Red Γ (.guard p `0 b) `0
+----------------------------------------------------------------
+---- Mapping Rules
+----------------------------------------------------------------
+| ctor1_map :
+  Red Γ (.ctor1 v (c1 ⊕ c2)) (.ctor1 v c1 ⊕ .ctor1 v c2)
+| ctor2_map1 :
+  ctor2_has_congr1 v ->
+  Red Γ (.ctor2 v (c1 ⊕ c2) t2) (.ctor2 v c1 t2 ⊕ .ctor2 v c2 t2)
+| ctor2_map2 :
+  ctor2_has_congr2 v ->
+  Red Γ (.ctor2 v t1 (c1 ⊕ c2)) (.ctor2 v t1 c1 ⊕ .ctor2 v t1 c2)
+| bind2_map1 :
+  bind2_has_congr1 v ->
+  Red Γ (.bind2 v (c1 ⊕ c2) t2) (.bind2 v c1 t2 ⊕ .bind2 v c2 t2)
+| bind2_map2 :
+  bind2_has_congr2 v ->
+  Red Γ (.bind2 v t1 (c1 ⊕ c2)) (.bind2 v t1 c1 ⊕ .bind2 v t1 c2)
+| ite_map :
+  Red Γ (.ite p (c1 ⊕ c2) b e) (.ite p c1 b e ⊕ .ite p c2 b e)
+| guard_map :
+  Red Γ (.guard p (c1 ⊕ c2) b) (.guard p c1 b ⊕ .guard p c2 b)
 
-inductive ListRed : Ctx Term -> List Term -> List Term -> Prop where
-| head : Red Γ h htl -> ListRed Γ (h::tl) (htl ++ tl)
-| tail : ListRed Γ tl tl' -> ListRed Γ (h::tl) (h::tl')
-
-inductive ListRedStar : Ctx Term -> List Term -> List Term -> Prop where
-| refl : ListRedStar Γ x x
-| step : ListRedStar Γ x y -> ListRed Γ y z -> ListRedStar Γ x z
+inductive RedStar : Ctx Term -> Term -> Term -> Prop where
+| refl : RedStar Γ x x
+| step : RedStar Γ x y -> Red Γ y z -> RedStar Γ x z
