SystemFD/Term/Definition.lean
@@ -1,12 +1,12 @@
 
 inductive Ctor1Variant : Type where
-| refl
 | sym
 | fst
 | snd
 deriving Repr
 
 inductive Ctor2Variant : Type where
+| refl
 | arrowk
 | appk
 | appt
@@ -15,7 +15,7 @@ inductive Ctor2Variant : Type where
 | seq
 | appc
 | apptc
-| eq
+| choice
 deriving Repr
 
 inductive Bind2Variant : Type where
@@ -31,9 +31,11 @@ inductive Term : Type where
 | kind : Term -- □
 | var : Nat -> Term
 | type : Term -- ★
+| zero : Term
 | ctor1 : Ctor1Variant -> Term -> Term
 | ctor2 : Ctor2Variant -> Term -> Term -> Term
 | bind2 : Bind2Variant -> Term -> Term -> Term
+| eq : Term -> Term -> Term -> Term
 | ite : Term   -- pattern
       -> Term  -- scrutinee
       -> Term  -- branch
@@ -50,12 +52,13 @@ protected def Term.repr (a : Term) (p : Nat): Std.Format :=
   | .kind => "□"
   | .var n => "#" ++ Nat.repr n
   | .type => "★"
+  | .zero => "0"
 
-  | .ctor1 .refl t => "≮" ++ Term.repr t p ++ "≯"
   | .ctor1 .sym t => "(sym! " ++ Term.repr t p ++ "!)"
   | .ctor1 .fst t => "(" ++ Term.repr t p ++ ")●1"
   | .ctor1 .snd t => "(" ++ Term.repr t p ++ ")●2"
 
+  | .ctor2 .refl t1 t2 => "(refl! " ++ Term.repr t1 p ++ "; " ++ Term.repr t2 p ++ ")"
   | .ctor2 .arrowk t1 t2 => Term.repr t1 p ++ Std.Format.line ++" → " ++ Term.repr t2 p
   | .ctor2 .appk t1 t2 => Std.Format.paren (Term.repr t1 p ++ " `@k " ++ Term.repr t2 p)
   | .ctor2 .appc t1 t2 => Std.Format.paren (Term.repr t1 p ++ " `@c " ++ Term.repr t2 p)
@@ -64,7 +67,7 @@ protected def Term.repr (a : Term) (p : Nat): Std.Format :=
   | .ctor2 .app t1 t2 => Std.Format.paren (Term.repr t1 p ++ " ⬝ " ++ Std.Format.line ++ Term.repr t2 p)
   | .ctor2 .cast t1 t2 => Std.Format.paren (Term.repr t1 p  ++ " ▹ "  ++ Std.Format.line ++ Term.repr t2 p)
   | .ctor2 .seq t1 t2 => Term.repr t1 p ++ " `; "  ++ Std.Format.line ++ Term.repr t2 p
-  | .ctor2 .eq t1 t2 => Term.repr t1 p ++ " ∼ " ++ Term.repr t2 p
+  | .ctor2 .choice t1 t2 => Term.repr t1 p ++ " ⊕ " ++ Term.repr t2 p
 
   | .bind2 .all t1 t2 => "∀" ++ Std.Format.sbracket (Term.repr t1 p) ++ Repr.addAppParen (Term.repr t2 p) p
   | .bind2 .arrow t1 t2 => Term.repr t1 p ++ " → " ++ Term.repr t2 p
@@ -73,6 +76,7 @@ protected def Term.repr (a : Term) (p : Nat): Std.Format :=
   | .bind2 .lamt t1 t2 => "Λ" ++ Std.Format.sbracket (Term.repr t1 p) ++ Repr.addAppParen (Term.repr t2 p) p
   | .bind2 .lam t1 t2 => "`λ" ++ Std.Format.sbracket (Term.repr t1 p) ++ Std.Format.line ++ Term.repr t2 p
 
+  | .eq t1 t2 t3 => Term.repr t1 p ++ " ∼[" ++ Term.repr t2 p ++ "]~ " ++ Term.repr t3 p
   | .ite pat s b c =>
          " match " ++ Term.repr s p ++ " with " ++
           Repr.addAppParen (Term.repr pat p) p ++ " ⇒ " ++ Term.repr b p ++ " | "
@@ -93,24 +97,27 @@ notation:14 a " -k> " b => Term.ctor2 Ctor2Variant.arrowk a b
 notation:14 a " -t> " b => Term.bind2 Bind2Variant.arrow a b
 notation:14 a " -c> " b => Term.bind2 Bind2Variant.arrowc a b
 notation "∀[" A "]" B => Term.bind2 Bind2Variant.all A B
-infixl:15 " `@k " => Term.ctor2 Ctor2Variant.appk
-infixl:15 " `@t " => Term.ctor2 Ctor2Variant.appt
-infixl:15 " `@ " => Term.ctor2 Ctor2Variant.app
+notation:15 t1:15 " `@k " t2:16 => Term.ctor2 Ctor2Variant.appk t1 t2
+notation:15 t1:15 " `@t " t2:16 => Term.ctor2 Ctor2Variant.appt t1 t2
+notation:15 t1:15 " `@ " t2:16 => Term.ctor2 Ctor2Variant.app t1 t2
 notation "Λ[" A "]" t => Term.bind2 Bind2Variant.lamt A t
 notation "`λ[" A "]" t => Term.bind2 Bind2Variant.lam A t
-infixl:15 " ▹ " => Term.ctor2 Ctor2Variant.cast
+notation:15 t1:16 " ▹ " t2:15 => Term.ctor2 Ctor2Variant.cast t1 t2
 prefix:max "#" => Term.var
 notation "∀c[" A "]" B => Term.bind2 Bind2Variant.allc A B
-infixl:15 " `; " => Term.ctor2 Ctor2Variant.seq
-infixl:15 " `@c " => Term.ctor2 Ctor2Variant.appc
+notation:15 t1:15 " `; " t2:16 => Term.ctor2 Ctor2Variant.seq t1 t2
+notation:15 t1:15 " `@c " t2:16 => Term.ctor2 Ctor2Variant.appc t1 t2
 notation:15 f:15 " `@c[" a "]" => Term.ctor2 Ctor2Variant.apptc f a
-infixl:15 " ~ " => Term.ctor2 Ctor2Variant.eq
+notation:15 A:15 " ~[" K "]~ " B:15 => Term.eq K A B
 notation:15 "If " p " ← " s " then " i " else " e => Term.ite p s i e
 
-prefix:max "refl! " => Term.ctor1 Ctor1Variant.refl
+prefix:max "refl! " => Term.ctor2 Ctor2Variant.refl
 prefix:max "sym! " => Term.ctor1 Ctor1Variant.sym
 postfix:max ".!1" => Term.ctor1 Ctor1Variant.fst
 postfix:max ".!2" => Term.ctor1 Ctor1Variant.snd
+
+notation "`0" => Term.zero
+notation:20 t1:20 " ⊕ " t2:20 => Term.ctor2 Ctor2Variant.choice t1 t2
 
 namespace Term
   @[simp]
@@ -118,9 +125,11 @@ namespace Term
   | var _ => 0
   | kind => 0
   | type => 0
+  | zero => 0
   | ctor1 _ t => (size t) + 1
   | ctor2 _ t1 t2 => (size t1) + (size t2) + 1
   | bind2 _ t1 t2 => (size t1) + (size t2) + 1
+  | eq t1 t2 t3 => (size t1) + (size t2) + (size t3) + 1
   | ite t1 t2 t3 t4 => (size t1) + (size t2) + (size t3) + (size t4) + 1
   | guard t1 t2 t3 => (size t1) + (size t2) + (size t3) + 1
   | letterm t1 t2 t3 => (size t1) + (size t2) + (size t3) + 1
