SystemFD.lean
@@ -1,27 +1,27 @@
 
 import SystemFD.Metatheory.TypeMatch
+import SystemFD.Metatheory.FrameWf
 import SystemFD.Metatheory.Weaken
 import SystemFD.Metatheory.Substitution
+import SystemFD.Metatheory.Shape
 import SystemFD.Metatheory.Uniqueness
 import SystemFD.Metatheory.Inversion
 import SystemFD.Metatheory.Classification
-import SystemFD.Metatheory.FrameWf
+import SystemFD.Metatheory.Canonicity
 import SystemFD.Metatheory.Preservation
 import SystemFD.Metatheory.Progress
-import SystemFD.Metatheory.Canonicity
 
-import SystemFD.Evaluator.Soundness
-import SystemFD.Evaluator
+-- import SystemFD.Evaluator.Soundness
+-- import SystemFD.Evaluator
 
-import SystemFD.Algorithm
-import SystemFD.Algorithm.TypeMatch
-import SystemFD.Algorithm.Soundness1
-import SystemFD.Algorithm.Soundness2
+-- import SystemFD.Algorithm
+-- import SystemFD.Algorithm.TypeMatch
+-- import SystemFD.Algorithm.Soundness1
+-- import SystemFD.Algorithm.Soundness2
 
-
-import SystemFD.Examples.Boolean
-import SystemFD.Examples.Maybe
-import SystemFD.Examples.Nat
-import SystemFD.Examples.Fundeps
-import SystemFD.Examples.TypeFunction
-import SystemFD.Examples.SuperClasses
+-- import SystemFD.Examples.Boolean
+-- import SystemFD.Examples.Maybe
+-- import SystemFD.Examples.Nat
+-- import SystemFD.Examples.Fundeps
+-- import SystemFD.Examples.TypeFunction
+-- import SystemFD.Examples.SuperClasses
