SystemFD/Metatheory/Shape.lean
@@ -1,0 +1,506 @@
+
+import SystemFD.Term
+import SystemFD.Term.Definition
+import SystemFD.Judgment
+import SystemFD.Ctx
+import SystemFD.Metatheory.Classification
+
+theorem super_kind_equal_subst : □ = [σ]t -> t = □ ∨ (∃ i, ∃ v, σ i = .su v ∧ v = □ ∧ t = #i) := by
+intro h; induction t generalizing σ <;> simp at *
+case _ x =>
+  generalize zdef : σ x = z at *
+  cases z <;> simp at *
+  case _ v =>
+    subst h; apply Exists.intro x
+    apply Exists.intro □; simp [*]
+
+theorem super_kind_equal_beta : □ = b β[t] -> b = □ ∨ (t = □ ∧ b = #0) := by
+intro h; have lem := super_kind_equal_subst h
+cases lem
+case _ lem => apply Or.inl lem
+case _ lem =>
+cases lem; case _ i lem =>
+cases lem; case _ v lem =>
+cases lem; case _ lem1 lem2 =>
+cases lem2; case _ lem2 lem3 =>
+  subst lem2; subst lem3; cases i <;> simp at *
+  subst h; rfl
+
+@[simp]
+abbrev SuperKindShapeLemmaType (Γ : Ctx Term) : (v : JudgmentVariant) -> JudgmentArgs v -> Prop
+| .prf => λ (t, A) => ¬ Term.Subexpr □ t ∧ (A = □ ∨ ¬ Term.Subexpr □ A)
+| .wf => λ () => ∀ n T, .some T = (Γ d@ n).get_type -> ¬ Term.Subexpr □ T
+
+macro "super_kind_shape_lemma_ctx_nil_case!" ih:term : tactic => `(tactic| {
+  intro n T h
+  cases n <;> simp at *
+  case _ =>
+    rw [<-Frame.get_type_apply_commute] at h
+    have lem := Frame.get_type_apply_eq_destruct h
+    cases lem; case _ T' lem =>
+    cases lem; case _ e lem =>
+      unfold Frame.get_type at lem; simp at lem
+  case _ n =>
+    rw [<-Frame.get_type_apply_commute] at h
+    have lem := Frame.get_type_apply_eq_destruct h
+    cases lem; case _ T' lem =>
+    cases lem; case _ e lem =>
+      subst e; have lem2 := $ih _ _ lem
+      intro h; apply lem2
+      apply Term.subexpr_from_rename (λ x => x + 1) h (by simp) (by simp)
+})
+
+macro "super_kind_shape_lemma_ctx_cons_case!" ih1:term "," ih2:term : tactic => `(tactic| {
+  intro n T h
+  cases n <;> simp at *
+  case _ =>
+    unfold Frame.get_type at h; simp at h
+    subst h; intro h
+    replace h := Term.subexpr_from_rename (λ x => x + 1) h (by simp) (by simp)
+    try (apply $ih2.1; assumption)
+    try (apply $ih2; assumption)
+  case _ n =>
+    rw [<-Frame.get_type_apply_commute] at h
+    have lem := Frame.get_type_apply_eq_destruct h
+    cases lem; case _ T' lem =>
+    cases lem; case _ e lem =>
+      subst e; have lem2 := $ih1 _ _ lem
+      intro h; apply lem2
+      apply Term.subexpr_from_rename (λ x => x + 1) h (by simp) (by simp)
+})
+
+theorem super_kind_shape_lemma : Judgment v Γ a -> SuperKindShapeLemmaType Γ v a := by
+intro j; induction j <;> simp at *
+case _ =>
+  intro T h; unfold Frame.get_type at h
+  simp at h
+case _ j ih => super_kind_shape_lemma_ctx_nil_case! ih
+case _ ih1 ih2 => super_kind_shape_lemma_ctx_cons_case! ih1 , ih2
+case _ ih1 ih2 => super_kind_shape_lemma_ctx_cons_case! ih1 , ih2
+case _ ih1 ih2 => super_kind_shape_lemma_ctx_cons_case! ih1 , ih2
+case _ ih1 ih2 => super_kind_shape_lemma_ctx_cons_case! ih1 , ih2
+case _ ih1 ih2 => super_kind_shape_lemma_ctx_cons_case! ih1 , ih2
+case _ ih1 ih2 => super_kind_shape_lemma_ctx_cons_case! ih1 , ih2
+case _ ih1 ih2 => super_kind_shape_lemma_ctx_cons_case! ih1 , ih2
+case _ ih1 ih2 => super_kind_shape_lemma_ctx_nil_case! ih2
+case _ ih1 ih2 ih3 => super_kind_shape_lemma_ctx_cons_case! ih2 , ih3
+case _ ih1 ih2 ih3 ih4 =>
+  apply And.intro; intro h; cases h
+  apply ih3.1; assumption
+  apply ih1.1; assumption
+  case _ s' q1 q2 =>
+    have lem : [P]□ = [P][S]s' := by rw [q1]
+    simp at lem; rw [<-lem] at q2
+    apply ih2.1; assumption
+  apply Or.inr ih4.1
+case _ => intro h; cases h
+case var x T j1 j2 ih =>
+  apply And.intro; intro h; cases h
+  replace ih := ih x T j2
+  apply Or.inr ih
+case _ ih1 ih2 =>
+  intro h; cases h
+  apply ih1; assumption
+  apply ih2; assumption
+case _ ih1 ih2 =>
+  apply And.intro; intro h; cases h
+  apply ih1; assumption
+  case _ s' q1 q2 =>
+    have lem : [P]□ = [P][S]s' := by rw [q1]
+    simp at lem; rw [<-lem] at q2
+    apply ih2.1; assumption
+  intro h; cases h
+case _ ih1 ih2 =>
+  apply And.intro; intro h; cases h
+  apply ih1.1; assumption
+  case _ s' q1 q2 =>
+    have lem : [P]□ = [P][S]s' := by rw [q1]
+    simp at lem; rw [<-lem] at q2
+    apply ih2.1; assumption
+  intro h; cases h
+case _ ih1 ih2 =>
+  apply And.intro; intro h; cases h
+  apply ih2.1; assumption
+  apply ih1.1; assumption
+  replace ih2 := Term.not_subexpr_ctor2 ih2.2
+  apply Or.inr ih2.2
+case _ ih1 ih2 ih3 =>
+  apply And.intro; intro h; cases h
+  apply ih3; assumption
+  apply ih1.1; assumption
+  apply ih2.1; assumption
+  intro h; cases h
+case _ ih1 ih2 ih3 ih4 ih5 ih6 ih7 =>
+  apply And.intro; intro h; cases h
+  apply ih2.1; assumption
+  apply ih3.1; assumption
+  apply ih4.1; assumption
+  apply ih5.1; assumption
+  apply Or.inr ih7.1
+case _ ih1 ih2 ih3 ih4 ih5 =>
+  apply And.intro; intro h; cases h
+  apply ih1.1; assumption
+  apply ih2.1; assumption
+  apply ih3.1; assumption
+  apply Or.inr; apply ih5.1
+case _ ih1 ih2 ih3 =>
+  apply And.intro; intro h; cases h
+  apply ih2.1; assumption
+  case _ s' q1 q2 =>
+    have lem : [P]□ = [P][S]s' := by rw [q1]
+    simp at lem; rw [<-lem] at q2
+    apply ih1.1; assumption
+  apply ih3.1
+case _ e ih1 ih2 =>
+  apply And.intro; intro h; cases h
+  apply ih2.1; assumption
+  apply ih1.1; assumption
+  have lem : □ = [S]□ := by simp
+  rw [lem] at ih2
+  replace ih2 := Term.not_subexpr_bind2 ih2.2
+  subst e; apply Or.inr; intro h
+  replace h := Term.subexpr_from_beta h (by simp) (by simp)
+  cases h
+  case _ h => apply ih2.2 h
+  case _ h => apply ih1.1 h
+case _ ih1 ih2 ih3 =>
+  apply And.intro; intro h; cases h
+  apply ih2; assumption
+  case _ s' q1 q2 =>
+    have lem : [P]□ = [P][S]s' := by rw [q1]
+    simp at lem; rw [<-lem] at q2
+    apply ih1.1; assumption
+  apply ih3.1
+case _ e ih1 ih2 =>
+  apply And.intro; intro h; cases h
+  apply ih2.1; assumption
+  apply ih1.1; assumption
+  have lem : □ = [S]□ := by simp
+  rw [lem] at ih2
+  replace ih2 := Term.not_subexpr_bind2 ih2.2
+  subst e; apply Or.inr; intro h
+  replace h := Term.subexpr_from_beta h (by simp) (by simp)
+  cases h
+  case _ h => apply ih2.2 h
+  case _ h => apply ih1.1 h
+case _ ih1 ih2 =>
+  apply And.intro; intro h; cases h
+  apply ih1.1; assumption
+  apply ih2.1; assumption
+  replace ih2 := Term.not_subexpr_eq ih2.2
+  apply Or.inr ih2.2.2
+case _ ih1 ih2 =>
+  apply And.intro; intro h; cases h
+  apply ih2; assumption
+  apply ih1.1; assumption
+  intro h; cases h
+  apply ih2; assumption
+  apply ih1.1; assumption
+  apply ih1.1; assumption
+case _ ih =>
+  apply And.intro; intro h; cases h
+  apply ih.1; assumption
+  replace ih := Term.not_subexpr_eq ih.2
+  intro h; cases h
+  apply ih.1; assumption
+  apply ih.2.2; assumption
+  apply ih.2.1; assumption
+case _ ih1 ih2 =>
+  apply And.intro; intro h; cases h
+  apply ih1.1; assumption
+  apply ih2.1; assumption
+  replace ih1 := Term.not_subexpr_eq ih1.2
+  replace ih2 := Term.not_subexpr_eq ih2.2
+  intro h; cases h
+  apply ih1.1; assumption
+  apply ih1.2.1; assumption
+  apply ih2.2.2; assumption
+case _ ih1 ih2 =>
+  apply And.intro; intro h; cases h
+  apply ih1.1; assumption
+  apply ih2.1; assumption
+  replace ih1 := Term.not_subexpr_eq ih1.2
+  replace ih2 := Term.not_subexpr_eq ih2.2
+  intro h; cases h
+  case _ h =>
+    apply ih1.1
+    apply Term.Subexpr.ctor2_2; assumption
+  case _ h =>
+    cases h
+    apply ih1.2.1; assumption
+    apply ih2.2.1; assumption
+  case _ h =>
+    cases h
+    case _ h =>
+      apply ih1.2.2; assumption
+    case _ h =>
+      apply ih2.2.2; assumption
+case _ ih1 ih2 =>
+  have lem1 := Term.not_subexpr_eq ih1.2
+  have lem2 := Term.not_subexpr_eq ih2.2
+  apply And.intro; intro h
+  cases h; apply ih1.1; assumption
+  case _ s' q1 q2 =>
+    have lem : [P]□ = [P][S]s' := by rw [q1]
+    simp at lem; rw [<-lem] at q2
+    apply ih2.1; assumption
+  intro h; cases h
+  case _ h => cases h
+  case _ h =>
+    cases h
+    apply lem1.2.1; assumption
+    case _ s' q1 q2 =>
+      have lem : [P]□ = [P][S]s' := by rw [q1]
+      simp at lem; rw [<-lem] at q2
+      apply lem2.2.1; assumption
+  case _ h =>
+    cases h
+    apply lem1.2.2; assumption
+    case _ s' q1 q2 =>
+      have lem : [P]□ = [P][S]s' := by rw [q1]
+      simp at lem; rw [<-lem] at q2
+      apply lem2.2.2; assumption
+case _ ih1 ih2 ih3 =>
+  apply And.intro; intro h; cases h
+  apply ih3.1; assumption
+  intro h; cases h
+  apply ih1.2; assumption
+  apply ih1.1; assumption
+  apply ih2.1; assumption
+case _ ih1 ih2 ih3 ih4 =>
+  apply And.intro; intro h; cases h
+  apply ih4.1; assumption
+  intro h; cases h
+  apply ih3; assumption
+  apply ih1.1; assumption
+  apply ih2.1; assumption
+case _ ih1 ih2 ih3 =>
+  have lem2 := Term.not_subexpr_eq ih3.2
+  apply And.intro; intro h; cases h
+  apply ih2; assumption
+  case _ s' q1 q2 =>
+    have lem : [P]□ = [P][S]s' := by rw [q1]
+    simp at lem; rw [<-lem] at q2
+    apply ih3.1; assumption
+  intro h; cases h
+  case _ h => cases h
+  case _ h =>
+    cases h
+    apply ih2; assumption
+    case _ s' q1 q2 =>
+      have lem : [P]□ = [P][S]s' := by rw [q1]
+      simp at lem; rw [<-lem] at q2
+      apply lem2.2.1; assumption
+  case _ h =>
+    cases h
+    apply ih2; assumption
+    case _ s' q1 q2 =>
+      have lem : [P]□ = [P][S]s' := by rw [q1]
+      simp at lem; rw [<-lem] at q2
+      apply lem2.2.2; assumption
+case _ e1 e2 ih1 ih2 =>
+  have lem0 : □ = [S]□ := by simp
+  have lem1 := Term.not_subexpr_eq ih1.2
+  have lem2 := Term.not_subexpr_eq ih2.2
+  rw [lem0] at lem1
+  have lem3 := Term.not_subexpr_bind2 lem1.2.1
+  have lem4 := Term.not_subexpr_bind2 lem1.2.2
+  simp at *
+  apply And.intro; intro h; cases h
+  apply ih1.1; assumption
+  apply ih2.1; assumption
+  intro h; cases h
+  case _ h => cases h
+  case _ h =>
+    rw [e1] at h
+    replace h := Term.subexpr_from_beta h (by simp) (by simp)
+    cases h
+    apply lem3.2; assumption
+    apply lem2.2.1; assumption
+  case _ h =>
+    rw [e2] at h
+    replace h := Term.subexpr_from_beta h (by simp) (by simp)
+    cases h
+    apply lem4.2; assumption
+    apply lem2.2.2; assumption
+case _ ih =>
+  apply And.intro; intro h; cases h
+  apply Or.inr; apply ih.1
+case _ ih1 ih2 ih3 =>
+  apply And.intro; intro h; cases h
+  apply ih1.1; assumption
+  apply ih2.1; assumption
+  apply Or.inr ih3.1
+
+@[simp]
+abbrev KindShapeLemmaType (_ : Ctx Term) : (v : JudgmentVariant) -> JudgmentArgs v -> Prop
+| .prf => λ (t, A) => A = □ -> Term.IsKind t
+| .wf => λ () => True
+
+macro "kind_shape_lemma_app_case!" j1:term "," j2:term " , " j3:term : tactic => `(tactic| {
+  intro h; subst h
+  replace j3 := super_kind_equal_beta $j3
+  cases j3
+  case _ h =>
+    subst h
+    have lem := super_kind_shape_lemma $j1; simp at lem
+    exfalso; apply lem.2
+    apply @Term.Subexpr.bind2_2 _ □; simp
+    constructor
+  case _ h =>
+    cases h; case _ e1 e2 =>
+      subst e1; subst e2
+      replace j2 := $j2
+      cases j2
+})
+
+theorem kind_shape_lemma : Judgment v Γ a -> KindShapeLemmaType Γ v a := by
+intro j; induction j <;> simp at *
+case _ j1 j2 j3 j4 ih1 ih2 ih3 ih4 =>
+  intro h; rw [h] at j4
+  cases j4
+case _ => constructor
+case _ j1 j2 _ =>
+  intro h; subst h
+  have lem := super_kind_shape_lemma j1; simp at lem
+  exfalso; apply lem _ _ j2
+  constructor
+case _ ih1 ih2 => constructor; assumption; assumption
+case _ j1 j2 _ _ =>
+  intro h; subst h
+  have lem := super_kind_shape_lemma j1; simp at lem
+  exfalso; apply lem.2
+  apply Term.Subexpr.ctor2_2
+  constructor
+case _ j1 j2 ih1 ih2 ih3 ih4 ih5 ih6 =>
+  intro h; rw [h] at j1; cases j1
+case _ j1 j2 ih1 ih2 ih3 ih4 ih5 =>
+  intro h; rw [h] at j2; cases j2
+case _ j1 j2 j3 _ _ => kind_shape_lemma_app_case! j1, j2, j3
+case _ j1 j2 j3 _ _ => kind_shape_lemma_app_case! j1, j2, j3
+case _ j _ _ =>
+  intro h; subst h
+  have lem := super_kind_shape_lemma j; simp at lem
+  exfalso; apply lem.2
+  apply Term.Subexpr.eq3
+  constructor
+case _ j _ =>
+  intro h; rw [h] at j
+  cases j
+case _ j1 j2 j3 ih1 ih2 ih3 =>
+  intro h; rw [h] at j1
+  cases j1
+
+theorem kind_shape : Γ ⊢ t : A -> A = □ -> Term.IsKind t := by
+intro j1 j2
+apply kind_shape_lemma j1 j2
+
+
+@[simp]
+abbrev TypeShapeLemmaType (_ : Ctx Term) : (v : JudgmentVariant) -> JudgmentArgs v -> Prop
+| .prf => λ (t, A) => Term.IsKind A -> Term.IsType t
+| .wf => λ () => True
+
+theorem type_shape_lemma : Judgment v Γ a -> TypeShapeLemmaType Γ v a := by
+intro j <;> induction j <;> simp at *
+case _ ih =>
+  intro h; replace ih := ih (by constructor)
+  exfalso; apply Term.is_kind_disjoint_is_type h ih
+case _ => intro h; cases h
+case _ => intro h; constructor
+case _ => intro h; cases h
+case _ j _ ih1 ih2 =>
+  intro h; have lem := kind_shape j rfl
+  constructor; apply lem
+  apply ih2 h
+case _ ih1 ih2 =>
+  intro h; constructor
+  apply ih1 h; apply ih2 h
+case _ f A B a j1 j2 ih1 ih2 =>
+  intro h
+  have lem := classification_lemma j1; simp at lem
+  cases lem
+  case _ lem =>
+    have lem2 := kind_shape lem rfl
+    replace ih1 := ih1 lem2
+    cases lem2; case _ q1 q2 =>
+      replace ih2 := ih2 q1
+      apply Term.IsType.app ih1 ih2
+  case _ lem =>
+    cases lem; case _ K lem =>
+    cases lem.2; cases lem.1
+case _ j1 j2 j3 ih1 ih2 ih3 =>
+  intro h
+  have lem := kind_shape j1 rfl
+  constructor; apply lem
+  apply ih2 lem; apply ih3 lem
+case _ j _ _ _ _ _ _ _ =>
+  intro h; cases h
+  cases j; cases j
+case _ j _ _ _ _ _ =>
+  intro h; cases h
+  cases j; cases j
+case _ => intro h; cases h
+case _ Γ f A B a B' j1 j2 j3 ih1 ih2 =>
+  intro h
+  have lem1 := classification_lemma j1; simp at lem1
+  cases lem1; case _ lem1 => cases lem1
+  case _ lem1 =>
+  cases lem1; case _ K lem1 =>
+  cases lem1; case _ lem1 lem2 =>
+  cases lem2; case _ q1 q2 =>
+    have lem3 : B.IsKind ∨ a.IsKind := by
+      subst j3; have lem := Term.is_kind_from_beta h
+      apply Or.comm.1 lem
+    cases lem3
+    case _ lem3 => cases lem3; cases q2; cases q2
+    case _ lem3 =>
+      cases lem3
+      case _ => cases j2; cases q1
+      case _ => cases j2; cases q1
+case _ => intro h; cases h
+case _ Γ f A B a B' j1 j2 j3 ih1 ih2 =>
+  intro h
+  have lem1 := classification_lemma j1; simp at lem1
+  cases lem1; case _ lem1 => cases lem1
+  case _ lem1 =>
+  cases lem1; case _ K lem1 =>
+  cases lem1; case _ lem1 lem2 =>
+  cases lem2; case _ q1 q2 =>
+    have lem3 : B.IsKind ∨ a.IsKind := by
+      subst j3; have lem := Term.is_kind_from_beta h
+      apply Or.comm.1 lem
+    cases lem3
+    case _ lem3 => cases lem3; cases q2; cases q2
+    case _ lem3 =>
+      cases lem3
+      case _ => cases j2; cases q1
+      case _ => cases j2; cases q1
+case _ Γ t A c K B j1 j2 ih1 ih2  =>
+  intro h
+  have lem1 := classification_lemma j2; simp at lem1
+  cases lem1; case _ lem1 => cases lem1
+  case _ lem1 =>
+  cases lem1; case _ K1 lem1 =>
+  cases lem1; case _ lem1 lem2 =>
+    cases h; cases lem2; case _ q1 q2 q3 => cases q3; cases q1
+    cases lem2; case _ q1 q2 q3 => cases q3; cases q1
+case _ => intro h; cases h
+case _ => intro h; cases h
+case _ => intro h; cases h
+case _ => intro h; cases h
+case _ => intro h; cases h
+case _ => intro h; cases h
+case _ => intro h; cases h
+case _ => intro h; cases h
+case _ => intro h; cases h
+case _ j _ =>
+  intro h; cases h
+  cases j; cases j
+case _ j _ _ _ _ _ =>
+  intro h; cases h
+  cases j; cases j
+
+theorem type_shape : Γ ⊢ t : A -> A.IsKind -> t.IsType := by
+intro j1 j2
+apply type_shape_lemma j1 j2
