SystemFD/Metatheory/Uniqueness.lean
@@ -3,22 +3,83 @@ import SystemFD.Term
 import SystemFD.Term.Definition
 import SystemFD.Judgment
 import SystemFD.Ctx
+import SystemFD.Metatheory.TypeMatch
+import SystemFD.Metatheory.Shape
+import SystemFD.Metatheory.Classification
 
-theorem no_valid_head_variable_with_all :
-  ¬ ValidHeadVariable (∀[A]B) test
+theorem uniqueness_of_super_kind :
+  t.IsKind -> Γ ⊢ t : A -> Γ ⊢ t : B -> A = B
 := by
-intro h; unfold ValidHeadVariable at h
-cases h; case _ x h =>
-cases h; case _ h1 h2 =>
-  simp at h1
+intro h1 j1 j2
+induction t generalizing Γ A B
+case _ => cases j1
+case _ x => cases h1
+case _ => cases j1; cases j2; rfl
+case _ => cases h1
+case _ => cases h1
+case _ v t1 t2 ih1 ih2 =>
+  cases h1
+  case _ h1 h2 =>
+    cases j1; case _ q1 q2 =>
+    cases j2; case _ r1 r2 =>
+      rfl
+case _ v t1 t2 ih1 ih2 => cases h1
+case _ =>
+  cases j1; case _ q1 q2 q3 =>
+  cases j2; case _ r1 r2 r3 =>
+    rfl
+case _ => cases h1
+case _ => cases h1
+case _ => cases h1
 
-theorem no_valid_head_variable_with_arrow :
-  ¬ ValidHeadVariable (A -t> B) test
+theorem uniqueness_of_kinds :
+  t.IsType -> Γ ⊢ t : A -> Γ ⊢ t : B -> A = B
 := by
-intro h; unfold ValidHeadVariable at h
-cases h; case _ x h =>
-cases h; case _ h1 h2 =>
-  simp at h1
+intro h1 j1 j2
+induction t generalizing Γ A B
+case _ => cases j1
+case _ x =>
+  cases j1; case _ q1 q2 =>
+  cases j2; case _ r1 r2 =>
+    generalize fdef : Γ d@ x = f at *
+    unfold Frame.get_type at *
+    cases f <;> simp at *
+    all_goals (subst q2; subst r2; rfl)
+case _ => cases j1; cases j2; rfl
+case _ => cases h1
+case _ => cases h1
+case _ v t1 t2 ih1 ih2 =>
+  cases h1
+  case _ h1 h2 =>
+    cases j1; case _ q =>
+    cases j2; case _ r =>
+      have lem := classification_lemma q <;> simp at lem
+      cases lem
+      case _ lem =>
+        have lem1 := kind_shape lem rfl
+        have lem2 := type_shape q lem1
+        replace ih1 := ih1 lem2 q r
+        injection ih1 with _ e1 e2
+      case _ lem =>
+        cases lem; case _ _ lem =>
+        cases lem.2; cases lem.1
+case _ v t1 t2 ih1 ih2 =>
+  cases h1
+  case _ h1 h2 =>
+    cases j1; case _ q1 =>
+    cases j2; case _ q2 =>
+      rfl
+  case _ h1 h2 =>
+    cases j1; case _ q1 =>
+    cases j2; case _ q2 =>
+      rfl
+case _ =>
+  cases j1; case _ q1 q2 q3 =>
+  cases j2; case _ r1 r2 r3 =>
+    rfl
+case _ => cases h1
+case _ => cases h1
+case _ => cases h1
 
 theorem uniqueness_prefix_match :
   PrefixTypeMatch Γ U V A ->
@@ -74,10 +135,10 @@ case _ v t1 t2 ih1 ih2 =>
       have lem : [P][S]A = [P][S]B := by rw [ih2]
       simp at lem; apply lem
 
-theorem uniqueness_of_types :
-  Γ ⊢ t : A -> Γ ⊢ t : B -> A = B
+theorem uniqueness_modulo_zero :
+  ¬ Term.Subexpr `0 t -> Γ ⊢ t : A -> Γ ⊢ t : B -> A = B
 := by
-intro j1 j2
+intro js j1 j2
 induction t generalizing Γ A B
 case _ => cases j1
 case _ x =>
@@ -88,85 +149,108 @@ case _ x =>
     cases f <;> simp at *
     all_goals (subst q2; subst r2; rfl)
 case _ => cases j1; cases j2; rfl
+case _ =>
+  exfalso; apply js; apply Term.Subexpr.refl
 case _ v t ih =>
+  replace js := Term.not_subexpr_ctor1 js
   cases v
-  case _ =>
-    cases j1; case _ K1 q1 q2 =>
-    cases j2; case _ K2 r1 r2 =>
-      rfl
   case _ =>
     cases j1; case _ A1 B1 q1 =>
     cases j2; case _ A2 B2 q2 =>
-      replace ih := ih q1 q2
-      injection ih with _ e1 e2
-      subst e1; subst e2; rfl
+      replace ih := ih js q1 q2
+      injection ih with e1 e2 e3
+      subst e1; subst e2; subst e3; rfl
   case _ =>
-    cases j1; case _ K1 q1 q2 =>
-    cases j2; case _ K2 r1 r2 =>
-      replace ih := ih q2 r2
-      injection ih with _ e1 e2
-      injection e1 with _ v1 v2
-      injection e2 with _ u1 u2
-      subst v1; subst v2; subst u1; subst u2
-      rfl
+    cases j1; case _ q1 q2 q3 =>
+    cases j2; case _ r1 r2 r3 =>
+      have lem1 := ih js q3 r3
+      injection lem1 with e1 e2 e3; subst e1
+      injection e2 with _ w1 w2; subst w1; subst w2
+      injection e3 with _ w1 w2; subst w1; subst w2
+      have lem2 := classification_lemma q1; simp at lem2
+      cases lem2
+      case _ lem2 =>
+        have lem3 := kind_shape lem2 rfl
+        have lem4 := type_shape q1 lem3
+        have lem5 := uniqueness_of_kinds lem4 q1 r1
+        injection lem5 with _ e1 e2; subst e1
+        rfl
+      case _ lem2 =>
+        cases lem2; case _ lem2 =>
+          cases lem2.2; cases lem2.1
   case _ =>
-    cases j1; case _ q1 =>
-    cases j2; case _ q2 =>
-      replace ih := ih q1 q2
-      injection ih with _ e1 e2
-      injection e1 with _ u1 u2
-      injection e2 with _ v1 v2
-      subst u1; subst u2; subst v1; subst v2
-      rfl
+    cases j1; case _ q1 q2 q3 q4 =>
+    cases j2; case _ r1 r2 r3 r4 =>
+      have lem1 := ih js q4 r4
+      injection lem1 with e1 e2 e3; subst e1
+      injection e2 with _ w1 w2; subst w1; subst w2
+      injection e3 with _ w1 w2; subst w1; subst w2
+      have lem2 := classification_lemma q2; simp at lem2
+      cases lem2; case _ h => subst h; cases q1
+      case _ lem2 =>
+      cases lem2; case _ lem2 =>
+        have lem3 := type_shape q2 (kind_shape lem2 rfl)
+        have lem4 := uniqueness_of_kinds lem3 q2 r2
+        subst lem4; rfl
+      case _ lem2 =>
+        cases lem2; case _ _ lem2 =>
+          have lem3 := uniqueness_of_super_kind (kind_shape q1 rfl) q1 lem2.2
+          subst lem3; cases lem2.1
 case _ v t1 t2 ih1 ih2 =>
+  replace js := Term.not_subexpr_ctor2 js
   cases v
   case _ =>
+    cases j1; case _ q1 q2 =>
+    cases j2; case _ r1 r2 =>
+      rfl
+  case _ =>
     cases j1; case _ q =>
     cases j2; case _ r =>
       rfl
   case _ =>
     cases j1; case _ q =>
     cases j2; case _ r =>
-      replace ih1 := ih1 q r
+      replace ih1 := ih1 js.1 q r
       injection ih1 with _ e1 e2
   case _ =>
     cases j1; case _ q1 q2 q3 =>
     cases j2; case _ r1 r2 r3 =>
-      replace ih1 := ih1 q1 r1
+      replace ih1 := ih1 js.1 q1 r1
       injection ih1 with _ e1 e2; subst e1; subst e2
       subst q3; subst r3; rfl
   case _ =>
     cases j1; case _ q1 q2 q3 =>
     cases j2; case _ r1 r2 r3 =>
-      replace ih1 := ih1 q1 r1
+      replace ih1 := ih1 js.1 q1 r1
       injection ih1 with _ e1 e2; subst e1; subst e2
       subst q3; subst r3; rfl
   case _ =>
     cases j1; case _ q =>
     cases j2; case _ r =>
-      replace ih2 := ih2 q r
+      replace ih2 := ih2 js.2 q r
       injection ih2 with _ e1 e2
   case _ =>
     cases j1; case _ q1 q2 =>
     cases j2; case _ r1 r2 =>
-      replace ih1 := ih1 q1 r1
-      replace ih2 := ih2 q2 r2
-      injection ih1 with _ e1 e2; subst e1; subst e2
-      injection ih2 with _ e1 e2; subst e2
+      replace ih1 := ih1 js.1 q1 r1
+      replace ih2 := ih2 js.2 q2 r2
+      injection ih1 with e3 e1 e2; subst e1; subst e2
+      injection ih2 with _ e1 e2; subst e2; subst e3
       rfl
   case _ =>
     cases j1; case _ q1 q2 =>
     cases j2; case _ r1 r2 =>
-      replace ih1 := ih1 q1 r1
-      replace ih2 := ih2 q2 r2
-      injection ih1 with _ e1 e2; subst e1; subst e2
+      replace ih1 := ih1 js.1 q1 r1
+      replace ih2 := ih2 js.2 q2 r2
+      injection ih1 with e3 e1 e2; subst e1; subst e2
       injection ih2 with _ e1 e2; subst e1; subst e2
+      injection e3 with _ e1 e2; subst e1; subst e2
       rfl
   case _ =>
     cases j1; case _ q1 q2 =>
     cases j2; case _ r1 r2 =>
-      replace ih1 := ih1 q1 r1
-      replace ih2 := ih2 q2 r2
+      replace ih1 := ih1 js.1 q1 r1
+      replace ih2 := ih2 js.2 q2 r2
       injection ih1 with _ e1 e2;
       injection e1 with _ w1 w2; subst w1; subst w2
       injection e2 with _ _ w1; subst w1
@@ -175,8 +259,11 @@ case _ v t1 t2 ih1 ih2 =>
   case _ =>
     cases j1; case _ q =>
     cases j2; case _ r =>
-      rfl
+      apply ih2 js.2 q r
 case _ v t1 t2 ih1 ih2 =>
+  have lem : `0 = [S]`0 := by simp
+  rw [lem] at js
+  replace js := Term.not_subexpr_bind2 js; simp at js
   cases v
   case _ =>
     cases j1; case _ q1 =>
@@ -185,12 +272,12 @@ case _ v t1 t2 ih1 ih2 =>
   case _ =>
     cases j1; case _ q1 =>
     cases j2; case _ q2 =>
-      replace ih2 := ih2 q1 q2; subst ih2
+      replace ih2 := ih2 js.2 q1 q2; subst ih2
       rfl
   case _ =>
     cases j1; case _ q1 =>
     cases j2; case _ q2 =>
-      replace ih2 := ih2 q1 q2; subst ih2
+      replace ih2 := ih2 js.2 q1 q2; subst ih2
       rfl
   case _ =>
     cases j1; case _ q1 =>
@@ -199,30 +286,74 @@ case _ v t1 t2 ih1 ih2 =>
   case _ =>
     cases j1; case _ q1 =>
     cases j2; case _ q2 =>
-      replace ih2 := ih2 q1 q2
+      replace ih2 := ih2 js.2 q1 q2
       injection ih2 with _ e1 e2
       subst e1; subst e2; rfl
   case _ =>
     cases j1; case _ q1 q2 q3 =>
     cases j2; case _ r1 r2 r3 =>
-      replace ih1 := ih1 q2 r2
-      replace ih2 := ih2 q3 r3
+      replace ih1 := ih1 js.1 q2 r2
+      replace ih2 := ih2 js.2 q3 r3
       injection ih1 with _ e1 e2; subst e1; subst e2
       injection ih2 with _ e1 e2; subst e1; subst e2
       rfl
+case _ ih1 ih2 ih3 =>
+  replace js := Term.not_subexpr_eq js
+  cases j1; case _ q1 q2 q3 =>
+  cases j2; case _ r1 r2 r3 =>
+    rfl
 case _ ih1 ih2 ih3 ih4 =>
+  replace js := Term.not_subexpr_ite js
   cases j1; case _ q1 =>
   cases j2; case _ r1 =>
-    replace ih4 := ih4 q1 r1; subst ih4; rfl
+    replace ih4 := ih4 js.2.2.2 q1 r1; subst ih4; rfl
 case _ ih1 ih2 ih3 =>
+  replace js := Term.not_subexpr_guard js
   cases j1; case _ q1 q2 q3 q4 q5 q6 =>
   cases j2; case _ r1 r2 r3 r4 r5 r6 =>
-    replace ih1 := ih1 q1 r1; subst ih1
-    replace ih3 := ih3 q4 r4; subst ih3
+    replace ih1 := ih1 js.1 q1 r1; subst ih1
+    replace ih3 := ih3 js.2.2 q4 r4; subst ih3
     apply uniqueness_prefix_match q5 r5
 case _ ih1 ih2 =>
+  have lem : `0 = [S]`0 := by simp
+  rw [lem] at js
+  replace js := Term.not_subexpr_letterm js; simp at js
   cases j1; case _ q1 =>
   cases j2; case _ r1 =>
-    replace ih2 := ih2 q1 r1;
+    replace ih2 := ih2 js.2.2 q1 r1;
     have lem : [P][S]A = [P][S]B := by rw [ih2]
     simp at lem; apply lem
+
+theorem type_disjoint :
+  Γ ⊢ t : A -> Γ ⊢ A : .kind ->
+  ¬ (A = .kind) ∧ ¬ (∃ K, Γ ⊢ K : .kind ∧ Γ ⊢ A : K)
+:= by
+intro j1 j2
+apply And.intro
+case _ =>
+  intro h; subst h; cases j2
+case _ =>
+  intro h
+  cases h; case _ K h =>
+  cases h; case _ h1 h2 =>
+    have lem1 := type_shape h2 (kind_shape h1 rfl)
+    have lem := uniqueness_of_kinds lem1 h2 j2; subst lem
+    cases h1
+
+theorem term_disjoint :
+  Γ ⊢ t : A -> (∃ K, Γ ⊢ K : .kind ∧ Γ ⊢ A : K) ->
+  ¬ (A = .kind) ∧ ¬ (Γ ⊢ A : .kind)
+:= by
+intro j1 j2
+have lem := classification_lemma j1; simp at lem
+cases j2; case _ K j2 =>
+cases j2; case _ j2 j2' =>
+  apply And.intro
+  case _ =>
+    intro h; subst h
+    cases j2'
+  case _ =>
+    intro h
+    have lem1 := type_shape j2' (kind_shape j2 rfl)
+    have lem := uniqueness_of_kinds lem1 j2' h; subst lem
+    cases j2
