SystemFD/Term.lean
@@ -3,3 +3,5 @@ import SystemFD.Term.Definition
 import SystemFD.Term.Equality
 import SystemFD.Term.Substitution
 import SystemFD.Term.Instances
+import SystemFD.Term.Subexpression
+import SystemFD.Term.Shape
