SystemFD/Term/Shape.lean
@@ -1,0 +1,70 @@
+import SystemFD.Term.Definition
+import SystemFD.Term.Substitution
+
+namespace Term
+
+  inductive IsKind : Term -> Prop where
+  | type : IsKind ★
+  | arrow : IsKind A -> IsKind B -> IsKind (A -k> B)
+
+  inductive IsType : Term -> Prop where
+  | var : IsType #x
+  | all : IsKind A -> IsType B -> IsType (∀[A] B)
+  | arrow : IsType A -> IsType B -> IsType (A -t> B)
+  | app : IsType A -> IsType B -> IsType (f `@k a)
+  | eq : IsKind K -> IsType A -> IsType B -> IsType (A ~[K]~ B)
+
+  theorem is_kind_disjoint_is_type : IsKind t -> ¬ IsType t := by
+  intro h1 h2
+  induction h1
+  all_goals (cases h2)
+
+  theorem zero_not_is_kind : ¬ IsKind `0 := by intro h; cases h
+
+  theorem zero_not_is_type : ¬ IsType `0 := by intro h; cases h
+
+  theorem is_kind_from_subst : IsKind ([σ]t) -> IsKind t ∨ (∃ i, ∃ v, σ i = .su v ∧ IsKind v) := by
+  intro h; induction t generalizing σ
+  all_goals simp at h; try cases h
+  case var x =>
+    generalize zdef : σ x = z at *
+    cases z <;> simp at *; cases h
+    case _ v =>
+      apply Or.inr; apply Exists.intro x
+      apply Exists.intro v
+      apply And.intro zdef h
+  case type => apply Or.inl; constructor
+  case arrow ih1 ih2 h1 h2 =>
+    replace ih1 := ih1 h1
+    replace ih2 := ih2 h2
+    cases ih1
+    case _ ih1 =>
+      cases ih2
+      case _ ih2 =>
+        apply Or.inl; constructor
+        assumption; assumption
+      case _ ih2 => apply Or.inr ih2
+    case _ ih1 => apply Or.inr ih1
+
+  theorem is_kind_from_beta : IsKind (b β[t]) -> IsKind t ∨ IsKind b := by
+  intro h
+  have lem := is_kind_from_subst h
+  cases lem; case _ lem => apply Or.inr lem
+  case _ lem =>
+  cases lem; case _ i lem =>
+  cases lem; case _ v lem =>
+  cases lem; case _ lem1 lem2 =>
+  cases i <;> simp at lem1
+  case _ => subst lem1; apply Or.inl lem2
+
+  theorem constant_non_variables_preserved_under_substitution σ :
+    t.size = 0 -> (∀ n, t ≠ #n) -> ([σ]t) = t
+  := by
+  intro h1 h2; induction t generalizing σ
+  all_goals simp
+  all_goals try solve | cases h1
+  case _ i =>
+    generalize zdef : σ i = z at *
+    cases z <;> simp at *
+
+end Term
