SystemFD/Term/VariableSet.lean
@@ -3,26 +3,26 @@ import SystemFD.Ctx
 import SystemFD.Term.Definition
 import SystemFD.Term.Substitution
 
-namespace List
-  @[simp]
-  def inter [BEq T] (l1 l2 : List T) : List T := filter (elem · l2) l1
-end List
+-- namespace List
+--   @[simp]
+--   def inter [BEq T] (l1 l2 : List T) : List T := filter (elem · l2) l1
+-- end List
 
-namespace Term
+-- namespace Term
 
-  @[simp]
-  def vars_inner (c : Nat) : Term -> List Nat
-  | var x => if c.ble x then [x - c] else []
-  | kind => []
-  | type => []
-  | ctor1 _ t => vars_inner c t
-  | ctor2 _ t1 t2 => vars_inner c t1 ++ vars_inner c t2
-  | bind2 _ t1 t2 => vars_inner c t1 ++ vars_inner (c + 1) t2
-  | ite t1 t2 t3 t4 => vars_inner c t1 ++ vars_inner c t2 ++ vars_inner c t3 ++ vars_inner c t4
-  | guard t1 t2 t3 => vars_inner c t1 ++ vars_inner c t2 ++ vars_inner c t3
-  | letterm t1 t2 t3 => vars_inner c t1 ++ vars_inner c t2 ++ vars_inner (c + 1) t3
+--   @[simp]
+--   def vars_inner (c : Nat) : Term -> List Nat
+--   | var x => if c.ble x then [x - c] else []
+--   | kind => []
+--   | type => []
+--   | ctor1 _ t => vars_inner c t
+--   | ctor2 _ t1 t2 => vars_inner c t1 ++ vars_inner c t2
+--   | bind2 _ t1 t2 => vars_inner c t1 ++ vars_inner (c + 1) t2
+--   | ite t1 t2 t3 t4 => vars_inner c t1 ++ vars_inner c t2 ++ vars_inner c t3 ++ vars_inner c t4
+--   | guard t1 t2 t3 => vars_inner c t1 ++ vars_inner c t2 ++ vars_inner c t3
+--   | letterm t1 t2 t3 => vars_inner c t1 ++ vars_inner c t2 ++ vars_inner (c + 1) t3
 
-  def vars (t : Term) : List Nat := vars_inner 0 t
+--   def vars (t : Term) : List Nat := vars_inner 0 t
 
   -- theorem zero_not_var_inner (r : Ren) (σ : Subst Term) :
   --   (∀ x, c ≤ x -> (x - c) ∉ Term.vars_inner c t) ->
@@ -47,4 +47,4 @@ namespace Term
   -- case _ => sorry
   -- case _ => sorry
 
-end Term
+-- end Term
